Testing Coq formatter

src/model/graph.v
@@ -1,1473 +1,1684 @@
 From Coq Require Import Lists.List.
+
 From Coq Require Import micromega.Lia.
+
 From Coq Require Import ZArith.ZArith.
 
 From VST Require Import floyd.proofauto.
 
 From CertiGraph Require Import graph.graph_model.
+
 From CertiGraph Require Import graph.graph_gen.
+
 From CertiGraph Require Import lib.EquivDec_ext.
+
 From CertiGraph Require Import lib.List_ext.
 
 From CertiGC Require Import model.constants.
+
 From CertiGC Require Import model.util.
 
 Import ListNotations.
-Local Coercion pg_lg: LabeledGraph >-> PreGraph.
 
+#[local]Coercion pg_lg : LabeledGraph >-> PreGraph.
 
-Record Addr: Type := {
-    addr_gen: nat;
-    addr_block: nat;
-}.
-Instance Addr_EqDec: EqDec Addr eq.
+Record Addr : Type :={ addr_gen  : nat; addr_block  : nat }.
+
+Instance Addr_EqDec : (EqDec Addr eq).
+
 Proof.
-    intros [gen_x block_x] [gen_y block_y].
-    destruct (equiv_dec gen_x gen_y) as [ H1 | H1 ] ;
-    destruct (equiv_dec block_x block_y) as [ H2 | H2 ].
-    all:
-      cbv in * ; subst ; try firstorder ;
-      right ; intro F ; congruence.
+  (intros [gen_x block_x] [gen_y block_y]).
+  (destruct (equiv_dec gen_x gen_y) as [H1| H1]; destruct (equiv_dec block_x block_y) as [H2| H2]).
+  all: (compute in *; subst; try firstorder; right; intro F; congruence).
 Defined.
 
+Record Field : Type :={ field_addr  : Addr; field_index  : nat }.
 
-Record Field: Type := {
-    field_addr: Addr;
-    field_index: nat;
-}.
-Instance Field_EqDec: EqDec Field eq.
+Instance Field_EqDec : (EqDec Field eq).
+
 Proof.
-    intros [addr_x index_x] [addr_y index_y].
-    destruct (equiv_dec addr_x addr_y) as [ H1 | H1 ] ;
-    destruct (equiv_dec index_x index_y) as [ H2 | H2 ].
-    all:
-      cbv in * ; subst ; try firstorder ;
-      right ; intro F ; congruence.
+  (intros [addr_x index_x] [addr_y index_y]).
+  (destruct (equiv_dec addr_x addr_y) as [H1| H1]; destruct (equiv_dec index_x index_y) as [H2| H2]).
+  all: (compute in *; subst; try firstorder; right; intro F; congruence).
 Defined.
 
+Inductive GC_Pointer :=
+    GCPtr : block -> ptrofs -> GC_Pointer.
 
-Inductive GC_Pointer := | GCPtr: block -> ptrofs -> GC_Pointer.
+Definition FieldValue : Type := option (Z + GC_Pointer).
 
-Definition FieldValue: Type := option (Z + GC_Pointer).
+Instance FieldValue_Inhabitant : (Inhabitant FieldValue) := None.
 
-Instance FieldValue_Inhabitant: Inhabitant FieldValue := None.
+Record Block : Type :=
+ {
+  block_mark  : bool;
+  block_copied_vertex  : Addr;
+  block_fields  : list FieldValue;
+  block_color  : Z;
+  block_tag  : Z;
+  block_tag__range  : (0 <= block_tag < 256)%Z;
+  block_color__range  : (0 <= block_color < 4)%Z;
+  block_fields__range  : (0 < Zlength block_fields < two_p (WORD_SIZE * 8 - 10))%Z;
+  block_tag__no_scan  : (NO_SCAN_TAG <= block_tag -> ~ In None block_fields)%Z
+ }.
 
-
-Record Block : Type := {
-    block_mark: bool;
-    block_copied_vertex: Addr;
-    block_fields: list FieldValue;
-    block_color: Z;
-    block_tag: Z;
-    block_tag__range: (0 <= block_tag < 256)%Z;
-    block_color__range: (0 <= block_color < 4)%Z;
-    block_fields__range: (0 < Zlength block_fields < two_p (WORD_SIZE * 8 - 10))%Z;
-    block_tag__no_scan: (NO_SCAN_TAG <= block_tag -> ~ In None block_fields)%Z;
-    (* TODO: what's up with this? why can raw_f be None at all? *)
-}.
-
-Lemma block_fields__range2: forall r,
-    Zlength (block_fields r) <= if Archi.ptr64 then Int64.max_signed else Int.max_signed.
+Lemma block_fields__range2 :
+  forall r, Zlength (block_fields r) <= (if Archi.ptr64 then Int64.max_signed else Int.max_signed).
 Proof.
-  intros. pose proof (block_fields__range r). remember (Zlength (block_fields r)).
-  clear Heqz. cbv delta[Archi.ptr64]. simpl. rewrite <- Z.lt_succ_r. destruct H.
-  transitivity (two_p (WORD_SIZE * 8 - 10)); auto. now vm_compute.
+  (intros).
+  (pose proof (block_fields__range r)).
+  (remember (Zlength (block_fields r))).
+  clear Heqz.
+  (cbv delta [Archi.ptr64]).
+  (simpl).
+  (rewrite <- Z.lt_succ_r).
+  (destruct H).
+  (transitivity (two_p (WORD_SIZE * 8 - 10)); auto).
+  now vm_compute.
 Qed.
 
-Lemma block_fields__not_nil (rvb: Block):
-    block_fields rvb <> nil.
+Lemma block_fields__not_nil (rvb : Block) : block_fields rvb <> nil.
 Proof.
-    pose proof (block_fields__range rvb) as H.
-    remember (block_fields rvb) as ff eqn:E.
-    clear E rvb.
-    now destruct ff.
+  (pose proof (block_fields__range rvb) as H).
+  (remember (block_fields rvb) as ff eqn:E ).
+  clear E rvb.
+  now destruct ff.
 Qed.
 
-Definition block_fields_head (rvb: Block): FieldValue
- := match block_fields rvb as l return (block_fields rvb = l -> FieldValue) with
+Definition block_fields_head 
+  (rvb : Block) : FieldValue :=
+  match block_fields rvb as l return (block_fields rvb = l -> FieldValue) with
+  | nil => fun E => False_rect _ (block_fields__not_nil _ E)
+  | f :: _ => fun _ => f
+  end eq_refl.
+
+Lemma block_fields_head__cons (rvb : Block) : exists f ff, block_fields rvb = f :: ff /\ block_fields_head rvb = f.
+Proof.
+  refine
+   (match block_fields rvb as l return (block_fields rvb = l -> _) with
     | nil => fun E => False_rect _ (block_fields__not_nil _ E)
-    | f :: _ => fun _ => f
-    end eq_refl.
-
-Lemma block_fields_head__cons (rvb: Block):
-    exists f ff, block_fields rvb = f :: ff /\ block_fields_head rvb = f.
-Proof.
-    refine (
-        match block_fields rvb as l return (block_fields rvb = l -> _) with
-        | nil => fun E => False_rect _ (block_fields__not_nil _ E)
-        | f :: ff => fun E => _
-        end eq_refl
-    ).
-    exists f, ff. destruct rvb. simpl in E. now subst.
+    | f :: ff => fun E => _
+    end eq_refl).
+  exists f,ff.
+  (destruct rvb).
+  (simpl in E).
+  now subst.
 Qed.
 
+Record Generation : Type :=
+ {
+  generation_base  : val;
+  generation_block_count  : nat;
+  generation_sh  : share;
+  generation_base__isptr  : isptr generation_base;
+  generation_sh__writable  : writable_share generation_sh
+ }.
 
-Record Generation: Type := {
-    generation_base: val;
-    generation_block_count: nat;
-    generation_sh: share;
-    generation_base__isptr: isptr generation_base;
-    generation_sh__writable: writable_share generation_sh;
-}.
-
-Definition null_generation: Generation := {|
+Definition null_generation : Generation :=
+  {|
     generation_base := Vptr xH Ptrofs.zero;
     generation_block_count := O;
     generation_sh := Tsh;
     generation_base__isptr := I;
-    generation_sh__writable := writable_share_top;
-|}.
+    generation_sh__writable := writable_share_top
+  |}.
 
-Instance Generation_Inhabitant: Inhabitant Generation := null_generation.
+Instance Generation_Inhabitant : (Inhabitant Generation) := null_generation.
 
+Record Generations : Type :={ generations  : list Generation; generations__not_nil  : generations <> nil }.
 
-Record Generations : Type := {
-    generations: list Generation;
-    generations__not_nil: generations <> nil;
-}.
-
-Definition generations_append (gi: Generations) (gen_i: Generation):
-    Generations
- := {|
-    generations := generations gi +:: gen_i;
-    generations__not_nil := app_not_nil (generations gi) gen_i;
-|}.
-
+Definition generations_append 
+  (gi : Generations) 
+  (gen_i : Generation) : Generations :=
+  {| generations := generations gi +:: gen_i; generations__not_nil := app_not_nil (generations gi) gen_i |}.
 
 Definition HeapGraph := LabeledGraph Addr Field Block unit Generations.
 
+Definition heapgraph_block (g : HeapGraph) (v : Addr) : Block := vlabel g v.
 
-Definition heapgraph_block (g: HeapGraph) (v: Addr):
-    Block
- := vlabel g v
-.
+Definition heapgraph_field_pairs 
+  (g : HeapGraph) (v : Addr) : 
+  list (Z + Addr * Z) :=
+  map (fun x => inr (v, Z.of_nat x)) (nat_inc_list (length (block_fields (heapgraph_block g v)))).
 
-
-Definition heapgraph_field_pairs (g: HeapGraph) (v: Addr):
-    list (Z + (Addr * Z))
- := map (fun x => inr (v, Z.of_nat x))
-        (nat_inc_list (length (block_fields (heapgraph_block g v))))
-.
-
-Lemma heapgraph_field_pairs__Zlength (g: HeapGraph) (v: Addr):
-    Zlength (heapgraph_field_pairs g v) = Zlength (block_fields (heapgraph_block g v)).
+Lemma heapgraph_field_pairs__Zlength 
+  (g : HeapGraph) (v : Addr) : 
+  Zlength (heapgraph_field_pairs g v) = Zlength (block_fields (heapgraph_block g v)).
 Proof.
-    unfold heapgraph_field_pairs.
-    now rewrite Zlength_map, !Zlength_correct, nat_inc_list_length.
+  (unfold heapgraph_field_pairs).
+  now rewrite Zlength_map, !Zlength_correct, nat_inc_list_length.
 Qed.
 
-Lemma heapgraph_field_pairs__Znth `[Inhabitant (Z + Addr * Z)]
-    (g: HeapGraph) (v: Addr) (i : Z)
-    (Hi: 0 <= i < Zlength (block_fields (heapgraph_block g v))):
-    Znth i (heapgraph_field_pairs g v) = inr (v, i).
+Lemma heapgraph_field_pairs__Znth 
+  `[Inhabitant (Z + Addr * Z)] 
+  (g : HeapGraph) (v : Addr) 
+  (i : Z) (Hi : 0 <= i < Zlength (block_fields (heapgraph_block g v))) :
+  Znth i (heapgraph_field_pairs g v) = inr (v, i).
 Proof.
-    unfold heapgraph_field_pairs.
-    assert (0 <= i < Zlength (nat_inc_list (length (block_fields (heapgraph_block g v)))))  as Hi'.
-    {
-        now rewrite Zlength_correct, nat_inc_list_length, <- Zlength_correct.
-    }
-    rewrite Znth_map by assumption.
-    do 2 f_equal.
-    rewrite <- nth_Znth by assumption.
-    rewrite nat_inc_list_nth.
-    {
-        rewrite Z2Nat.id ;  lia.
-    }
-    rewrite <- ZtoNat_Zlength, <- Z2Nat.inj_lt; lia.
+  (unfold heapgraph_field_pairs).
+  (assert (Hi' : 0 <= i < Zlength (nat_inc_list (length (block_fields (heapgraph_block g v)))))).
+  {
+    now rewrite Zlength_correct, nat_inc_list_length, <- Zlength_correct.
+  }
+  (rewrite Znth_map by assumption).
+  (do 2 f_equal).
+  (rewrite <- nth_Znth by assumption).
+  (rewrite nat_inc_list_nth).
+  {
+    (rewrite Z2Nat.id; lia).
+  }
+  (rewrite <- ZtoNat_Zlength, <- Z2Nat.inj_lt; lia).
 Qed.
 
+Definition heapgraph_block_size (g : HeapGraph) (v : Addr) : Z := Zlength (heapgraph_block g v).(block_fields) + 1.
 
-Definition heapgraph_block_size (g: HeapGraph) (v: Addr):
-    Z
- := Zlength (heapgraph_block g v).(block_fields) + 1
-.
-
-Lemma heapgraph_block_size__one (g: HeapGraph) (v: Addr):
-    1 < heapgraph_block_size g v.
+Lemma heapgraph_block_size__one (g : HeapGraph) (v : Addr) : 1 < heapgraph_block_size g v.
 Proof.
-    unfold heapgraph_block_size.
-    pose proof (block_fields__range (heapgraph_block g v)).
-    lia.
+  (unfold heapgraph_block_size).
+  (pose proof (block_fields__range (heapgraph_block g v))).
+  lia.
 Qed.
 
+Definition heapgraph_block_size_accum 
+  (g : HeapGraph) (gen : nat) 
+  (s : Z) (n : nat) : Z := 
+  s + heapgraph_block_size g {| addr_gen := gen; addr_block := n |}.
 
-Definition heapgraph_block_size_accum (g: HeapGraph) (gen: nat) (s: Z) (n: nat):
-    Z
- := s + heapgraph_block_size g {| addr_gen := gen; addr_block := n |}
-.
-
-Lemma heapgraph_block_size_accum__mono (g: HeapGraph) (gen: nat) (s: Z) (n: nat):
-    s < heapgraph_block_size_accum g gen s n.
+Lemma heapgraph_block_size_accum__mono 
+  (g : HeapGraph) (gen : nat) 
+  (s : Z) (n : nat) : 
+  s < heapgraph_block_size_accum g gen s n.
 Proof.
-    unfold heapgraph_block_size_accum.
-    pose proof (heapgraph_block_size__one g {| addr_gen := gen; addr_block := n |}) as H.
-    lia.
+  (unfold heapgraph_block_size_accum).
+  (pose proof (heapgraph_block_size__one g {| addr_gen := gen; addr_block := n |}) as H).
+  lia.
 Qed.
 
-Lemma heapgraph_block_size_accum__comm (g: HeapGraph) (gen: nat) (s: Z) (n1 n2: nat):
-    heapgraph_block_size_accum g gen (heapgraph_block_size_accum g gen s n1) n2 =
-    heapgraph_block_size_accum g gen (heapgraph_block_size_accum g gen s n2) n1.
+Lemma heapgraph_block_size_accum__comm 
+  (g : HeapGraph) (gen : nat) 
+  (s : Z) (n1 n2 : nat) :
+  heapgraph_block_size_accum g gen (heapgraph_block_size_accum g gen s n1) n2 =
+  heapgraph_block_size_accum g gen (heapgraph_block_size_accum g gen s n2) n1.
 Proof.
-    unfold heapgraph_block_size_accum.
-    lia.
+  (unfold heapgraph_block_size_accum).
+  lia.
 Qed.
 
-Lemma heapgraph_block_size_accum__fold_lt (g: HeapGraph) (gen: nat) (s: Z) (l: list nat)
-    (Hl: l <> nil):
-    s < fold_left (heapgraph_block_size_accum g gen) l s.
+Lemma heapgraph_block_size_accum__fold_lt 
+  (g : HeapGraph) (gen : nat) 
+  (s : Z) (l : list nat) 
+  (Hl : l <> nil) : s < fold_left (heapgraph_block_size_accum g gen) l s.
 Proof.
-    apply (fold_left_Z_mono_strict (heapgraph_block_size_accum g gen) nil l l) ; try assumption.
-    + apply heapgraph_block_size_accum__mono.
-    + apply heapgraph_block_size_accum__comm.
-    + apply Permutation_refl.
+  (apply (fold_left_Z_mono_strict (heapgraph_block_size_accum g gen) nil l l); try assumption).
+  + (apply heapgraph_block_size_accum__mono).
+  + (apply heapgraph_block_size_accum__comm).
+  + (apply Permutation_refl).
 Qed.
 
-Lemma heapgraph_block_size_accum__fold_le (g: HeapGraph) (gen: nat) (s: Z) (l: list nat):
-    s <= fold_left (heapgraph_block_size_accum g gen) l s.
+Lemma heapgraph_block_size_accum__fold_le 
+  (g : HeapGraph) (gen : nat) 
+  (s : Z) (l : list nat) : 
+  s <= fold_left (heapgraph_block_size_accum g gen) l s.
 Proof.
-    destruct l as [|n l] ; try easy.
-    rewrite Z.le_lteq.
+  (destruct l as [| n l]; try easy).
+  (rewrite Z.le_lteq).
+  left.
+  now apply heapgraph_block_size_accum__fold_lt.
+Qed.
+
+Lemma heapgraph_block_size_accum__fold_left 
+  (g : HeapGraph) (gen : nat) 
+  (l : list nat) (z1 z2 : Z) :
+  fold_left (heapgraph_block_size_accum g gen) l (z2 + z1) = fold_left (heapgraph_block_size_accum g gen) l z2 + z1.
+Proof.
+  (revert z1 z2; induction l as [| s l IHl]; intros z1 z2; simpl; try easy).
+  (rewrite <- IHl).
+  f_equal.
+  (unfold heapgraph_block_size_accum).
+  lia.
+Qed.
+
+Definition heapgraph_block_size_prev 
+  (g : HeapGraph) (gen i : nat) : Z := 
+  fold_left (heapgraph_block_size_accum g gen) (nat_inc_list i) 0.
+
+Lemma heapgraph_block_size_prev__S 
+  (g : HeapGraph) (gen i : nat) :
+  heapgraph_block_size_prev g gen (S i) =
+  heapgraph_block_size_prev g gen i + heapgraph_block_size g {| addr_gen := gen; addr_block := i |}.
+Proof.
+  (unfold heapgraph_block_size_prev at 1).
+  now rewrite nat_inc_list_S, fold_left_app.
+Qed.
+
+Lemma heapgraph_block_size_prev__nonneg (g : HeapGraph) (gen i : nat) : 0 <= heapgraph_block_size_prev g gen i.
+Proof.
+  (unfold heapgraph_block_size_prev).
+  (apply heapgraph_block_size_accum__fold_le).
+Qed.
+
+Lemma heapgraph_block_size_prev__mono_strict 
+  (g : HeapGraph) (gen i j : nat) 
+  (Hij : (i < j)%nat) : 
+  heapgraph_block_size_prev g gen i < heapgraph_block_size_prev g gen j.
+Proof.
+  (assert (Hij' : (j = i + (j - i))%nat) by lia).
+  (rewrite Hij').
+  (remember (j - i)%nat as n eqn:En ).
+  subst j.
+  (unfold heapgraph_block_size_prev).
+  (rewrite nat_inc_list_app, fold_left_app).
+  (apply heapgraph_block_size_accum__fold_lt).
+  (pose proof (nat_seq_length i n) as Hin).
+  (destruct (nat_seq i n); try easy).
+  (simpl in Hin).
+  lia.
+Qed.
+
+Lemma heapgraph_block_size_prev__mono 
+  (g : HeapGraph) (gen i j : nat) 
+  (Hij : (i <= j)%nat) : 
+  heapgraph_block_size_prev g gen i <= heapgraph_block_size_prev g gen j.
+Proof.
+  (rewrite Nat.le_lteq in Hij).
+  (destruct Hij as [Hij| Hij]).
+  + (rewrite Z.le_lteq).
     left.
-    now apply heapgraph_block_size_accum__fold_lt.
-Qed.
-
-Lemma heapgraph_block_size_accum__fold_left (g : HeapGraph) (gen : nat) (l : list nat) (z1 z2 : Z):
-    fold_left (heapgraph_block_size_accum g gen) l (z2 + z1) =
-    fold_left (heapgraph_block_size_accum g gen) l z2 + z1.
-Proof.
-    revert z1 z2 ; induction l as [| s l IHl] ; intros z1 z2 ; simpl ; try easy.
-    rewrite <- IHl.
-    f_equal.
-    unfold heapgraph_block_size_accum. lia.
-Qed.
-
-
-Definition heapgraph_block_size_prev (g: HeapGraph) (gen i: nat):
-    Z
- := fold_left (heapgraph_block_size_accum g gen) (nat_inc_list i) 0
-.
-
- Lemma heapgraph_block_size_prev__S (g: HeapGraph) (gen i: nat):
-    heapgraph_block_size_prev g gen (S i) =
-    heapgraph_block_size_prev g gen i + heapgraph_block_size g {| addr_gen := gen; addr_block := i |}.
-Proof.
-    unfold heapgraph_block_size_prev at 1.
-    now rewrite nat_inc_list_S, fold_left_app.
-Qed.
-
-Lemma heapgraph_block_size_prev__nonneg (g: HeapGraph) (gen i: nat):
-    0 <= heapgraph_block_size_prev g gen i.
-Proof.
-    unfold heapgraph_block_size_prev.
-    apply heapgraph_block_size_accum__fold_le.
-Qed.
-
-Lemma heapgraph_block_size_prev__mono_strict (g: HeapGraph) (gen i j: nat)
-    (Hij: (i < j)%nat):
-    (heapgraph_block_size_prev g gen i < heapgraph_block_size_prev g gen j).
-Proof.
-    assert (j = i + (j - i))%nat as Hij' by lia. rewrite Hij'.
-    remember (j - i)%nat as n eqn:En. subst j.
-    unfold heapgraph_block_size_prev. rewrite nat_inc_list_app, fold_left_app.
-    apply heapgraph_block_size_accum__fold_lt.
-    pose proof (nat_seq_length i n) as Hin.
-    destruct (nat_seq i n) ; try easy.
-    simpl in Hin. lia.
-Qed.
-
-Lemma heapgraph_block_size_prev__mono (g: HeapGraph) (gen i j: nat)
-    (Hij: (i <= j)%nat):
-    heapgraph_block_size_prev g gen i <= heapgraph_block_size_prev g gen j.
-Proof.
-    rewrite Nat.le_lteq in Hij.
-    destruct Hij as [Hij|Hij].
-    + rewrite Z.le_lteq. left. now apply heapgraph_block_size_prev__mono_strict.
-    + subst. lia.
-Qed.
-
-Lemma heapgraph_block_size_prev__lt_rev (g: HeapGraph) (gen i j: nat)
-    (Hij: heapgraph_block_size_prev g gen i < heapgraph_block_size_prev g gen j):
-    (i < j)%nat.
-Proof.
-    destruct (le_lt_dec j i) as [Hij'|Hij'] ; try easy.
-    apply (heapgraph_block_size_prev__mono g gen) in Hij'.
+    now apply heapgraph_block_size_prev__mono_strict.
+  + subst.
     lia.
 Qed.
 
-
-Definition heapgraph_generations (g: HeapGraph):
-    Generations
- := g.(glabel)
-.
-
-
-Definition heapgraph_generation (g: HeapGraph) (gen: nat):
-    Generation
- := nth gen (heapgraph_generations g).(generations) null_generation
-.
-
-
-Definition heapgraph_generation_block_count (g: HeapGraph) (gen: nat):
-    nat
- := generation_block_count (heapgraph_generation g gen)
-.
-
-Lemma heapgraph_generation_block_count__labeledgraph_gen_dst (g: HeapGraph) (e: Field) (v: Addr) (to: nat):
-    heapgraph_generation_block_count (labeledgraph_gen_dst g e v) to = heapgraph_generation_block_count g to.
-Proof. reflexivity. Qed.
-
-
-Definition heapgraph_generation_sh (g: HeapGraph) (gen: nat): share
- := generation_sh (heapgraph_generation g gen)
-.
-
-
-Definition heapgraph_has_gen (g: HeapGraph) (n: nat):
-    Prop
- := (n < length (heapgraph_generations g).(generations))%nat
-.
-
-Definition heapgraph_has_gen_dec g n:
-    {heapgraph_has_gen g n} + {~ heapgraph_has_gen g n}
- := lt_dec n (length (generations (heapgraph_generations g)))
-.
-
-Lemma heapgraph_has_gen__O (g: HeapGraph):
-    heapgraph_has_gen g O.
+Lemma heapgraph_block_size_prev__lt_rev 
+  (g : HeapGraph) (gen i j : nat) 
+  (Hij : heapgraph_block_size_prev g gen i < heapgraph_block_size_prev g gen j) : 
+  (i < j)%nat.
 Proof.
-    hnf.
-    destruct (generations (heapgraph_generations g)) as [|x xx] eqn:E ; simpl; try lia.
-    now pose proof (generations__not_nil (heapgraph_generations g)).
+  (destruct (le_lt_dec j i) as [Hij'| Hij']; try easy).
+  (apply (heapgraph_block_size_prev__mono g gen) in Hij').
+  lia.
 Qed.
 
+Definition heapgraph_generations (g : HeapGraph) : Generations := g.(glabel).
 
-Definition heapgraph_generation_has_index (g: HeapGraph) (gen index: nat):
-    Prop
- := (index < generation_block_count (heapgraph_generation g gen))%nat
-.
+Definition heapgraph_generation 
+  (g : HeapGraph) (gen : nat) : Generation := 
+  nth gen (heapgraph_generations g).(generations) null_generation.
 
+Definition heapgraph_generation_block_count 
+  (g : HeapGraph) (gen : nat) : nat := 
+  generation_block_count (heapgraph_generation g gen).
 
-Definition heapgraph_block_offset (g: HeapGraph) (v: Addr):
-  Z
- := heapgraph_block_size_prev g (addr_gen v) (addr_block v) + 1
-.
-
-
-Definition heapgraph_generation_size (g: HeapGraph) (gen: nat):
-    Z
- := heapgraph_block_size_prev g gen (generation_block_count (heapgraph_generation g gen))
-.
-
-Lemma heapgraph_block_offset__heapgraph_generation_size (g: HeapGraph) (v: Addr)
-    (Hgv: heapgraph_generation_has_index g (addr_gen v) (addr_block v)):
-    heapgraph_block_offset g v < heapgraph_generation_size g (addr_gen v).
+Lemma heapgraph_generation_block_count__labeledgraph_gen_dst 
+  (g : HeapGraph) (e : Field) 
+  (v : Addr) (to : nat) :
+  heapgraph_generation_block_count (labeledgraph_gen_dst g e v) to = heapgraph_generation_block_count g to.
 Proof.
-    unfold heapgraph_block_offset, heapgraph_generation_size. red in Hgv.
-    remember (generation_block_count (heapgraph_generation g (addr_gen v))) as n eqn:En.
-    remember (addr_gen v) as gen eqn:Egen.
-    assert (S (addr_block v) <= n)%nat by lia.
-    apply Z.lt_le_trans with (heapgraph_block_size_prev g gen (S (addr_block v))).
-    + rewrite heapgraph_block_size_prev__S. apply Zplus_lt_compat_l, heapgraph_block_size__one.
-    + now apply heapgraph_block_size_prev__mono.
+  reflexivity.
 Qed.
 
+Definition heapgraph_generation_sh (g : HeapGraph) (gen : nat) : share := generation_sh (heapgraph_generation g gen).
 
-Definition heapgraph_generations_append (g: HeapGraph) (gen_i: Generation):
-    HeapGraph
- := {|
+Definition heapgraph_has_gen 
+  (g : HeapGraph) (n : nat) : Prop := 
+  (n < length (heapgraph_generations g).(generations))%nat.
+
+Definition heapgraph_has_gen_dec 
+  g n : {heapgraph_has_gen g n} + {~ heapgraph_has_gen g n} :=
+  lt_dec n (length (generations (heapgraph_generations g))).
+
+Lemma heapgraph_has_gen__O (g : HeapGraph) : heapgraph_has_gen g O.
+Proof.
+  (hnf).
+  (destruct (generations (heapgraph_generations g)) as [| x xx] eqn:E; simpl; try lia).
+  now pose proof (generations__not_nil (heapgraph_generations g)).
+Qed.
+
+Definition heapgraph_generation_has_index 
+  (g : HeapGraph) (gen index : nat) : Prop := 
+  (index < generation_block_count (heapgraph_generation g gen))%nat.
+
+Definition heapgraph_block_offset 
+  (g : HeapGraph) (v : Addr) : Z := 
+  heapgraph_block_size_prev g (addr_gen v) (addr_block v) + 1.
+
+Definition heapgraph_generation_size 
+  (g : HeapGraph) (gen : nat) : Z :=
+  heapgraph_block_size_prev g gen (generation_block_count (heapgraph_generation g gen)).
+
+Lemma heapgraph_block_offset__heapgraph_generation_size 
+  (g : HeapGraph) (v : Addr) 
+  (Hgv : heapgraph_generation_has_index g (addr_gen v) (addr_block v)) :
+  heapgraph_block_offset g v < heapgraph_generation_size g (addr_gen v).
+Proof.
+  (unfold heapgraph_block_offset, heapgraph_generation_size).
+  (red in Hgv).
+  (remember (generation_block_count (heapgraph_generation g (addr_gen v))) as n eqn:En ).
+  (remember (addr_gen v) as gen eqn:Egen ).
+  (assert (S (addr_block v) <= n)%nat by lia).
+  (apply Z.lt_le_trans with (heapgraph_block_size_prev g gen (S (addr_block v)))).
+  + (rewrite heapgraph_block_size_prev__S).
+    (apply Zplus_lt_compat_l, heapgraph_block_size__one).
+  + now apply heapgraph_block_size_prev__mono.
+Qed.
+
+Definition heapgraph_generations_append 
+  (g : HeapGraph) (gen_i : Generation) : HeapGraph :=
+  {|
     pg_lg := pg_lg g;
     vlabel := heapgraph_block g;
     elabel := elabel g;
-    glabel := generations_append (heapgraph_generations g) gen_i;
-|}.
+    glabel := generations_append (heapgraph_generations g) gen_i
+  |}.
 
-Lemma heapgraph_has_gen__heapgraph_generations_append (g: HeapGraph) (gi: Generation) (gen: nat):
-    heapgraph_has_gen (heapgraph_generations_append g gi) gen <->
-    heapgraph_has_gen g gen \/ gen = length (generations (heapgraph_generations g)).
+Lemma heapgraph_has_gen__heapgraph_generations_append 
+  (g : HeapGraph) (gi : Generation) 
+  (gen : nat) :
+  heapgraph_has_gen (heapgraph_generations_append g gi) gen <->
+  heapgraph_has_gen g gen \/ gen = length (generations (heapgraph_generations g)).
 Proof.
-    unfold heapgraph_has_gen ; simpl.
-    rewrite app_length ; simpl.
+  (unfold heapgraph_has_gen; simpl).
+  (rewrite app_length; simpl).
+  lia.
+Qed.
+
+Lemma heapgraph_generation__heapgraph_generations_append__old 
+  (g : HeapGraph) (gi : Generation) 
+  (gen : nat) (Hgen : heapgraph_has_gen g gen) :
+  heapgraph_generation (heapgraph_generations_append g gi) gen = heapgraph_generation g gen.
+Proof.
+  (unfold heapgraph_generation; simpl).
+  now rewrite app_nth1.
+Qed.
+
+Lemma heapgraph_generation__heapgraph_generations_append__new 
+  (g : HeapGraph) (gi : Generation) :
+  heapgraph_generation (heapgraph_generations_append g gi) (length (generations (heapgraph_generations g))) = gi.
+Proof.
+  (unfold heapgraph_generation; simpl).
+  (rewrite app_nth2 by lia).
+  now rewrite Nat.sub_diag.
+Qed.
+
+Definition heapgraph_generation_base 
+  (g : HeapGraph) (gen : nat) : val :=
+  if heapgraph_has_gen_dec g gen then generation_base (heapgraph_generation g gen) else Vundef.
+
+Lemma heapgraph_generation_base__isptr 
+  (g : HeapGraph) (n : nat) 
+  (Hgn : heapgraph_has_gen g n) : 
+  isptr (heapgraph_generation_base g n).
+Proof.
+  (unfold heapgraph_generation_base).
+  (if_tac; try easy).
+  (apply generation_base__isptr).
+Qed.
+
+Definition heapgraph_block_ptr 
+  (g : HeapGraph) (v : Addr) : val :=
+  offset_val (WORD_SIZE * heapgraph_block_offset g v) (heapgraph_generation_base g (addr_gen v)).
+
+Lemma heapgraph_block_ptr__eq 
+  (g1 g2 : HeapGraph) 
+  (v : Addr) (Hv : forall v, heapgraph_block g1 v = heapgraph_block g2 v)
+  (Hg1g2 : map generation_base (heapgraph_generations g1).(generations) =
+           map generation_base (heapgraph_generations g2).(generations)) :
+  heapgraph_block_ptr g1 v = heapgraph_block_ptr g2 v.
+Proof.
+  (unfold heapgraph_block_ptr).
+  f_equal.
+  {
+    f_equal.
+    (unfold heapgraph_block_offset).
+    f_equal.
+    (remember (addr_block v) as n eqn:En ).
+    clear En.
+    (induction n as [| n IHn]; simpl; auto).
+    (rewrite !heapgraph_block_size_prev__S, IHn).
+    f_equal.
+    (unfold heapgraph_block_size).
+    now rewrite Hv.
+  }
+  {
+    (assert (Hgen : forall gen, heapgraph_has_gen g1 gen <-> heapgraph_has_gen g2 gen)).
+    {
+      intro gen.
+      (unfold heapgraph_has_gen).
+      (assert (E : length (generations (heapgraph_generations g1)) = length (generations (heapgraph_generations g2)))).
+      {
+        now rewrite <- !(map_length generation_base), Hg1g2.
+      }
+      lia.
+    }
+    (unfold heapgraph_generation_base).
+    (do 2 if_tac; rewrite Hgen in H; try easy).
+    (unfold heapgraph_generation).
+    now rewrite <- !(map_nth generation_base), Hg1g2.
+  }
+Qed.
+
+Definition heapgraph_block_header 
+  (g : HeapGraph) (v : Addr) : Z :=
+  let vb := heapgraph_block g v in
+  if vb.(block_mark) then 0 else vb.(block_tag) + Z.shiftl vb.(block_color) 8 + Z.shiftl (Zlength vb.(block_fields)) 10.
+
+Lemma heapgraph_block_header__iff 
+  (g : HeapGraph) (v : Addr) : 
+  heapgraph_block_header g v = 0 <-> block_mark (heapgraph_block g v) = true.
+Proof.
+  (unfold heapgraph_block_header).
+  (destruct (block_mark (heapgraph_block g v)); try easy).
+  (split; intro H; try easy).
+  (pose proof (proj1 (block_fields__range (heapgraph_block g v))) as Hfields).
+  (assert (F : Z.shiftl (Zlength (block_fields (heapgraph_block g v))) 10 = 0)).
+  {
+    (assert (Hshift__color : 0 <= Z.shiftl (block_color (heapgraph_block g v)) 8)).
+    {
+      (pose proof (proj1 (block_color__range (heapgraph_block g v))) as Hcolor).
+      now rewrite Z.shiftl_nonneg.
+    }
+    (pose proof (proj1 (block_tag__range (heapgraph_block g v))) as Htag).
+    (remember (Zlength (block_fields (heapgraph_block g v))) as z eqn:Ez ; clear Ez).
+    (assert (F' : 0 <= Z.shiftl z 10)).
+    {
+      (apply Z.shiftl_nonneg).
+      lia.
+    }
     lia.
+  }
+  (rewrite Z.shiftl_eq_0_iff in F; lia).
 Qed.
 
-Lemma heapgraph_generation__heapgraph_generations_append__old (g : HeapGraph) (gi : Generation) (gen : nat)
-    (Hgen: heapgraph_has_gen g gen):
-    heapgraph_generation (heapgraph_generations_append g gi) gen = heapgraph_generation g gen.
+Lemma heapgraph_block_header__range 
+  (g : HeapGraph) (v : Addr) : 
+  0 <= heapgraph_block_header g v < two_p (WORD_SIZE * 8).
 Proof.
-    unfold heapgraph_generation ; simpl.
-    now rewrite app_nth1.
+  (unfold heapgraph_block_header).
+  (destruct (block_mark (heapgraph_block g v))).
+  {
+    (pose proof (two_p_gt_ZERO (WORD_SIZE * 8))).
+    (unfold WORD_SIZE in *).
+    lia.
+  }
+  (pose proof (block_tag__range (heapgraph_block g v)) as Htag).
+  (pose proof (block_color__range (heapgraph_block g v)) as Hcolor).
+  (pose proof (block_fields__range (heapgraph_block g v)) as Hfields).
+  (remember (block_tag (heapgraph_block g v)) as z1 eqn:Ez1 ; clear Ez1).
+  (remember (block_color (heapgraph_block g v)) as z2 eqn:Ez2 ; clear Ez2).
+  (remember (Zlength (block_fields (heapgraph_block g v))) as z3 eqn:Ez3 ; clear Ez3).
+  (assert (Hz2 : 0 <= 8) by lia).
+  (apply (Zbits.Zshiftl_mul_two_p z2) in Hz2).
+  (rewrite Hz2).
+  clear Hz2.
+  (assert (Hz3 : 0 <= 10) by lia).
+  (apply (Zbits.Zshiftl_mul_two_p z3) in Hz3).
+  (rewrite Hz3).
+  clear Hz3.
+  (assert (Htwo_p10 : two_p 10 > 0) by (apply two_p_gt_ZERO; lia)).
+  (assert (Htwo_p8 : two_p 8 > 0) by (apply two_p_gt_ZERO; lia)).
+  split.
+  {
+    (assert (Hz2' : 0 <= z2 * two_p 8) by (apply Z.mul_nonneg_nonneg; lia)).
+    (assert (Hz3' : 0 <= z3 * two_p 10) by (apply Z.mul_nonneg_nonneg; lia)).
+    lia.
+  }
+  (change 256 with (two_p 8) in Htag).
+  (change 4 with (two_p 2) in Hcolor).
+  (assert (Hz1' : z1 <= two_p 8 - 1) by lia).
+  clear Htag.
+  (assert (Hz2' : z2 <= two_p 2 - 1) by lia).
+  clear Hcolor.
+  (assert (Hz3' : z3 <= two_p (WORD_SIZE * 8 - 10) - 1) by lia).
+  clear Hfields.
+  (apply Z.mul_le_mono_nonneg_r with (p := two_p 8) in Hz1'; try lia).
+  (apply Z.mul_le_mono_nonneg_r with (p := two_p 10) in Hz3'; try lia).
+  (rewrite Z.mul_sub_distr_r, Z.mul_1_l in Hz1', Hz3').
+  (assert (Hwordsize : 0 <= WORD_SIZE * 8 - 10) by (unfold WORD_SIZE; lia)).
+  (rewrite <- two_p_is_exp in Hz1', Hz3' by lia; clear Hwordsize).
+  (simpl Z.add in Hz1', Hz3').
+  Opaque two_p.
+  (simpl).
+  Transparent two_p.
+  (remember (two_p 2) as x eqn:E ; compute in E; subst x).
+  (remember (two_p 8) as x eqn:E ; compute in E; subst x).
+  (remember (two_p 10) as x eqn:E ; compute in E; subst x).
+  (remember (two_p 16) as x eqn:E ; compute in E; subst x).
+  (remember (two_p 64) as x eqn:E ; compute in E; subst x).
+  lia.
 Qed.
 
-Lemma heapgraph_generation__heapgraph_generations_append__new (g: HeapGraph) (gi: Generation):
-    heapgraph_generation (heapgraph_generations_append g gi) (length (generations (heapgraph_generations g))) = gi.
+Lemma heapgraph_block_header__repr_iff 
+  (g : HeapGraph) (v : Addr) :
+  (if Archi.ptr64
+   then Int64.repr (heapgraph_block_header g v) = Int64.repr 0
+   else Int.repr (heapgraph_block_header g v) = Int.repr 0) <-> 
+  block_mark (heapgraph_block g v) = true.
 Proof.
-    unfold heapgraph_generation ; simpl.
-    rewrite app_nth2 by lia.
-    now rewrite Nat.sub_diag.
+  (rewrite <- heapgraph_block_header__iff).
+  (split; intro H; [  | rewrite H; reflexivity ]).
+  (cbv delta [Archi.ptr64] in H).
+  (simpl in H).
+  Transparent Int.repr Int64.repr.
+  (inversion H).
+  Opaque Int64.repr Int.repr.
+  clear H.
+  (rewrite H1).
+  (match goal with
+   | H:Int64.Z_mod_modulus _ = _ |- _ => rewrite Int64.Z_mod_modulus_eq in H
+   | H:Int.Z_mod_modulus _ = _ |- _ => rewrite Int.Z_mod_modulus_eq in H
+   end).
+  (rewrite Z.mod_small in H1; auto).
+  (apply heapgraph_block_header__range).
 Qed.
 
-
-Definition heapgraph_generation_base (g: HeapGraph) (gen: nat):
-    val
- := if heapgraph_has_gen_dec g gen
-    then generation_base (heapgraph_generation g gen)
-    else Vundef
-.
-
-Lemma heapgraph_generation_base__isptr (g: HeapGraph) (n: nat)
-    (Hgn: heapgraph_has_gen g n):
-    isptr (heapgraph_generation_base g n).
+Lemma heapgraph_block_header__Wosize 
+  (g : HeapGraph) (v : Addr) 
+  (H : block_mark (heapgraph_block g v) = false) :
+  if Archi.ptr64
+  then
+   Int64.shru (Int64.repr (heapgraph_block_header g v)) (Int64.repr 10) =
+   Int64.repr (Zlength (block_fields (heapgraph_block g v)))
+  else
+   Int.shru (Int.repr (heapgraph_block_header g v)) (Int.repr 10) =
+   Int.repr (Zlength (block_fields (heapgraph_block g v))).
 Proof.
-    unfold heapgraph_generation_base.
-    if_tac ; try easy.
-    apply generation_base__isptr.
-Qed.
-
-
-Definition heapgraph_block_ptr (g: HeapGraph) (v: Addr):
-    val
- := offset_val
-      (WORD_SIZE * heapgraph_block_offset g v)
-      (heapgraph_generation_base g (addr_gen v))
-.
-
-Lemma heapgraph_block_ptr__eq (g1 g2: HeapGraph) (v: Addr)
-    (Hv: forall v, heapgraph_block g1 v = heapgraph_block g2 v)
-    (Hg1g2: map generation_base (heapgraph_generations g1).(generations) = map generation_base (heapgraph_generations g2).(generations)):
-    heapgraph_block_ptr g1 v = heapgraph_block_ptr g2 v.
-Proof.
-    unfold heapgraph_block_ptr. f_equal.
-    {
-      f_equal. unfold heapgraph_block_offset. f_equal.
-      remember (addr_block v) as n eqn:En. clear En.
-      induction n as [|n IHn] ; simpl ; auto.
-      rewrite !heapgraph_block_size_prev__S, IHn. f_equal.
-      unfold heapgraph_block_size.
-      now rewrite Hv.
-    }
-    {
-      assert (forall gen, heapgraph_has_gen g1 gen <-> heapgraph_has_gen g2 gen) as Hgen.
-      {
-        intro gen. unfold heapgraph_has_gen.
-        assert (length (generations (heapgraph_generations g1)) = length (generations (heapgraph_generations g2))) as E.
-        {
-          now rewrite <- !(map_length generation_base), Hg1g2.
-        }
-        lia.
-      }
-      unfold heapgraph_generation_base.
-      do 2 if_tac ; rewrite Hgen in H ; try easy.
-      unfold heapgraph_generation.
-      now rewrite <- !(map_nth generation_base), Hg1g2.
-    }
-Qed.
-
-
-Definition heapgraph_block_header (g: HeapGraph) (v: Addr):
-    Z
- := let vb := heapgraph_block g v
- in if vb.(block_mark)
-    then 0
-    else vb.(block_tag) + (Z.shiftl vb.(block_color) 8) + (Z.shiftl (Zlength vb.(block_fields)) 10).
-
-Lemma heapgraph_block_header__iff (g: HeapGraph) (v: Addr):
-    heapgraph_block_header g v = 0 <-> block_mark (heapgraph_block g v) = true.
-Proof.
-    unfold heapgraph_block_header. destruct (block_mark (heapgraph_block g v)) ; try easy.
-    split ; intro H ; try easy.
-    pose proof (proj1 (block_fields__range (heapgraph_block g v))) as Hfields.
-    assert (Z.shiftl (Zlength (block_fields (heapgraph_block g v))) 10 = 0) as F.
-    {
-      assert (0 <= Z.shiftl (block_color (heapgraph_block g v)) 8) as Hshift__color.
-      {
-        pose proof (proj1 (block_color__range (heapgraph_block g v))) as Hcolor.
-        now rewrite Z.shiftl_nonneg.
-      }
-      pose proof (proj1 (block_tag__range (heapgraph_block g v))) as Htag.
-      remember (Zlength (block_fields (heapgraph_block g v))) as z eqn:Ez ; clear Ez.
-      assert (0 <= Z.shiftl z 10) as F'.
-      {
-        apply Z.shiftl_nonneg.
-        lia.
-      }
-      lia.
-    }
-    rewrite Z.shiftl_eq_0_iff in F ; lia.
-Qed.
-
-Lemma heapgraph_block_header__range (g: HeapGraph) (v: Addr):
-    0 <= heapgraph_block_header g v < two_p (WORD_SIZE * 8).
-Proof.
-    unfold heapgraph_block_header. destruct (block_mark (heapgraph_block g v)).
-    {
-      pose proof (two_p_gt_ZERO (WORD_SIZE * 8)).
-      unfold WORD_SIZE in *.
-      lia.
-    }
-    pose proof (block_tag__range (heapgraph_block g v)) as Htag.
-    pose proof (block_color__range (heapgraph_block g v)) as Hcolor.
-    pose proof (block_fields__range (heapgraph_block g v)) as Hfields.
-    remember (block_tag (heapgraph_block g v)) as z1 eqn:Ez1 ; clear Ez1.
-    remember (block_color (heapgraph_block g v)) as z2 eqn:Ez2 ; clear Ez2.
-    remember (Zlength (block_fields (heapgraph_block g v))) as z3 eqn:Ez3 ; clear Ez3.
-    assert (0 <= 8) as Hz2 by lia. apply (Zbits.Zshiftl_mul_two_p z2) in Hz2. rewrite Hz2. clear Hz2.
-    assert (0 <= 10) as Hz3 by lia. apply (Zbits.Zshiftl_mul_two_p z3) in Hz3. rewrite Hz3. clear Hz3.
-    assert (two_p 10 > 0) as Htwo_p10 by (apply two_p_gt_ZERO; lia).
-    assert (two_p 8 > 0) as Htwo_p8 by (apply two_p_gt_ZERO; lia).
+  (cbv delta [Archi.ptr64]).
+  (simpl).
+  (match goal with
+   | |- Int64.shru _ _ = Int64.repr _ => rewrite Int64.shru_div_two_p, !Int64.unsigned_repr
+   | |- Int.shru _ _ = Int.repr _ => rewrite Int.shru_div_two_p, !Int.unsigned_repr
+   end).
+  - f_equal.
+    (unfold heapgraph_block_header).
+    (remember (heapgraph_block g v) as r eqn:E ).
+    clear E.
+    (rewrite H, !Zbits.Zshiftl_mul_two_p by lia).
+    (rewrite Z.div_add).
+    2: (compute; lia).
+    (pose proof (block_tag__range r)).
+    (pose proof (block_color__range r)).
+    (cut ((block_tag r + block_color r * two_p 8) / two_p 10 = 0)).
+    1: (intros; lia).
+    (apply Z.div_small).
+    (change 256 with (two_p 8) in H0).
+    (change 4 with (two_p 2) in H1).
+    (assert (0 <= block_tag r <= two_p 8 - 1) by lia).
+    clear H0.
+    (destruct H2).
+    (assert (0 <= block_color r <= two_p 2 - 1) by lia).
+    clear H1.
+    (destruct H3).
+    (assert (two_p 8 > 0) by (apply two_p_gt_ZERO; lia)).
     split.
-    {
-      assert (0 <= z2 * two_p 8) as Hz2' by (apply Z.mul_nonneg_nonneg; lia).
-      assert (0 <= z3 * two_p 10) as Hz3' by (apply Z.mul_nonneg_nonneg; lia).
+    + (assert (0 <= block_color r * two_p 8) by (apply Z.mul_nonneg_nonneg; lia)).
       lia.
-    }
-    change 256 with (two_p 8) in Htag.
-    change 4 with (two_p 2) in Hcolor.
-    assert (z1 <= two_p 8 - 1) as Hz1' by lia. clear Htag.
-    assert (z2 <= two_p 2 - 1) as Hz2' by lia. clear Hcolor.
-    assert (z3 <= two_p (WORD_SIZE * 8 - 10) - 1) as Hz3' by lia. clear Hfields.
-    apply Z.mul_le_mono_nonneg_r with (p := two_p 8) in Hz1' ; try lia.
-    apply Z.mul_le_mono_nonneg_r with (p := two_p 10) in Hz3' ; try lia.
-    rewrite Z.mul_sub_distr_r, Z.mul_1_l in Hz1', Hz3'.
-    assert (0 <= WORD_SIZE * 8 - 10) as Hwordsize by (unfold WORD_SIZE; lia).
-    rewrite <- two_p_is_exp in Hz1', Hz3' by lia ; clear Hwordsize.
-    simpl Z.add in Hz1', Hz3'.
-    Opaque two_p. simpl. Transparent two_p.
-    remember (two_p 2) as x eqn:E ; cbv in E ; subst x.
-    remember (two_p 8) as x eqn:E ; cbv in E ; subst x.
-    remember (two_p 10) as x eqn:E ; cbv in E ; subst x.
-    remember (two_p 16) as x eqn:E ; cbv in E ; subst x.
-    remember (two_p 64) as x eqn:E ; cbv in E ; subst x.
+    + (apply Z.mul_le_mono_nonneg_r with (p := two_p 8) in H3).
+      2: lia.
+      (rewrite Z.mul_sub_distr_r, <- two_p_is_exp in H3 by lia).
+      (simpl Z.add in H3).
+      lia.
+  - rep_lia.
+  - (pose proof (heapgraph_block_header__range g v)).
+    (unfold WORD_SIZE in *).
+    (match goal with
+     | |- context [ Int64.max_unsigned ] =>
+           unfold Int64.max_unsigned, Int64.modulus, Int64.wordsize, Wordsize_64.wordsize
+     | |- context [ Int.max_unsigned ] => unfold Int.max_unsigned, Int.modulus, Int.wordsize, Wordsize_32.wordsize
+     end).
+    (simpl Z.mul in H0).
+    (rewrite two_power_nat_two_p).
+    (simpl Z.of_nat).
     lia.
 Qed.
 
-Lemma heapgraph_block_header__repr_iff (g: HeapGraph) (v: Addr):
-    (if Archi.ptr64
-        then Int64.repr (heapgraph_block_header g v) = Int64.repr 0
-        else Int.repr (heapgraph_block_header g v) = Int.repr 0) <->
-    block_mark (heapgraph_block g v) = true.
+Definition Cell : Type := Z + GC_Pointer + Field.
+
+Instance Cell_inhabitant : (Inhabitant Cell) := (inl (inl Z.zero)).
+
+Definition GC_Pointer2val (x : GC_Pointer) : val := match x with
+                    | GCPtr b z => Vptr b z
+                    end.
+
+Definition heapgraph_cell_val 
+  (g : HeapGraph) (fd : Cell) : val :=
+  match fd with
+  | inl (inl z) => odd_Z2val z
+  | inl (inr p) => GC_Pointer2val p
+  | inr e => heapgraph_block_ptr g (dst g e)
+  end.
+
+Fixpoint fields_to_cells 
+(l_raw : list FieldValue) 
+(v : Addr) (n : nat) : 
+list Cell :=
+  match l_raw with
+  | nil => nil
+  | Some (inl z) :: l => inl (inl z) :: fields_to_cells l v (n + 1)
+  | Some (inr ptr) :: l => inl (inr ptr) :: fields_to_cells l v (n + 1)
+  | None :: l => inr {| field_addr := v; field_index := n |} :: fields_to_cells l v (n + 1)
+  end.
+
+Lemma fields_to_cells__in 
+  (l : list FieldValue) 
+  (v : Addr) (n : nat) 
+  (e : Field) (He : In (inr e) (fields_to_cells l v n)) : 
+  exists s, e = {| field_addr := v; field_index := s |}.
 Proof.
-    rewrite <- heapgraph_block_header__iff.
-    split ; intro H ; [|rewrite H; reflexivity].
-    cbv delta [Archi.ptr64] in H. simpl in H.
-    Transparent Int.repr Int64.repr. inversion H. Opaque Int64.repr Int.repr. clear H.
-    rewrite H1.
-    match goal with
-    | H : Int64.Z_mod_modulus _ = _ |- _ => rewrite Int64.Z_mod_modulus_eq in H
-    | H : Int.Z_mod_modulus _ = _ |- _ => rewrite Int.Z_mod_modulus_eq in H
-    end.
-    rewrite Z.mod_small in H1; auto.
-    apply heapgraph_block_header__range.
+  (revert v n e He; induction l as [| f l IHl]; intros v n e He; simpl in *; try easy).
+  (destruct f as [f| ]).
+  + (destruct f as [f| f]).
+    all: (destruct He as [He| He]; now try apply IHl with (n + 1)%nat).
+  + (destruct He as [He| He]).
+    - exists n.
+      congruence.
+    - now apply IHl with (n + 1)%nat.
 Qed.
 
-Lemma heapgraph_block_header__Wosize (g: HeapGraph) (v: Addr)
-    (H: block_mark (heapgraph_block g v) = false):
-    if Archi.ptr64
-    then
-      Int64.shru (Int64.repr (heapgraph_block_header g v)) (Int64.repr 10) =
-      Int64.repr (Zlength (block_fields (heapgraph_block g v)))
-    else
-      Int.shru (Int.repr (heapgraph_block_header g v)) (Int.repr 10) =
-      Int.repr (Zlength (block_fields (heapgraph_block g v))).
+Lemma fields_to_cells__length (l : list FieldValue) (v : Addr) (n : nat) : length (fields_to_cells l v n) = length l.
 Proof.
-    cbv delta [Archi.ptr64]. simpl.
-    match goal with
-    | |- Int64.shru _ _ = Int64.repr _ => rewrite Int64.shru_div_two_p, !Int64.unsigned_repr
-    | |- Int.shru _ _ = Int.repr _ => rewrite Int.shru_div_two_p, !Int.unsigned_repr
-    end.
-    - f_equal. unfold heapgraph_block_header.
-      remember (heapgraph_block g v) as r eqn:E. clear E.
-      rewrite H, !Zbits.Zshiftl_mul_two_p by lia. rewrite Z.div_add. 2: compute; lia.
-      pose proof (block_tag__range r). pose proof (block_color__range r).
-      cut ((block_tag r + block_color r * two_p 8) / two_p 10 = 0). 1: intros; lia.
-      apply Z.div_small. change 256 with (two_p 8) in H0. change 4 with (two_p 2) in H1.
-      assert (0 <= block_tag r <= two_p 8 - 1) by lia. clear H0. destruct H2.
-      assert (0 <= block_color r <= two_p 2 - 1) by lia. clear H1. destruct H3.
-      assert (two_p 8 > 0) by (apply two_p_gt_ZERO; lia). split.
-      + assert (0 <= block_color r * two_p 8) by (apply Z.mul_nonneg_nonneg; lia). lia.
-      + apply Z.mul_le_mono_nonneg_r with (p := two_p 8) in H3. 2: lia.
-        rewrite Z.mul_sub_distr_r, <- two_p_is_exp in H3 by lia. simpl Z.add in H3. lia.
-    - rep_lia.
-    - pose proof (heapgraph_block_header__range g v). unfold WORD_SIZE in *.
-      match goal with
-      | |- context [Int64.max_unsigned] =>
-        unfold Int64.max_unsigned, Int64.modulus, Int64.wordsize, Wordsize_64.wordsize
-      | |- context [Int.max_unsigned] =>
-        unfold Int.max_unsigned, Int.modulus, Int.wordsize, Wordsize_32.wordsize
-      end. simpl Z.mul in H0. rewrite two_power_nat_two_p. simpl Z.of_nat. lia.
+  (revert n; induction l as [| f l IHl]; intro n; simpl; try easy).
+  (destruct f as [f| ]; try destruct f as [f| f]; simpl).
+  all: now rewrite IHl.
 Qed.
 
-
-Definition Cell:
-    Type
- := Z + GC_Pointer + Field
-.
-
-Instance Cell_inhabitant: Inhabitant Cell := inl (inl Z.zero).
-
-Definition GC_Pointer2val (x: GC_Pointer):
-    val
- := match x with | GCPtr b z => Vptr b z end
-.
-
-Definition heapgraph_cell_val (g: HeapGraph) (fd: Cell):
-    val
- := match fd with
-    | inl (inl z) => odd_Z2val z
-    | inl (inr p) => GC_Pointer2val p
-    | inr e => heapgraph_block_ptr g (dst g e)
-    end
-.
-
-
-Fixpoint fields_to_cells (l_raw: list FieldValue) (v: Addr) (n: nat):
-    list Cell
- := match l_raw with
-    | nil => nil
-    | Some (inl z) :: l => inl (inl z) :: fields_to_cells l v (n + 1)
-    | Some (inr ptr) :: l => inl (inr ptr) :: fields_to_cells l v (n + 1)
-    | None :: l => inr {| field_addr := v; field_index := n |} :: fields_to_cells l v (n + 1)
-    end
-.
-
-Lemma fields_to_cells__in (l: list FieldValue) (v: Addr) (n: nat) (e: Field)
-    (He: In (inr e) (fields_to_cells l v n)):
-    exists s, e = {| field_addr := v; field_index := s |}.
+Lemma fields_to_cells__Zlength (l : list FieldValue) (v : Addr) (n : nat) : Zlength (fields_to_cells l v n) = Zlength l.
 Proof.
-    revert v n e He ; induction l as [|f l IHl] ; intros v n e He ; simpl in * ; try easy.
-    destruct f as [f|].
-    + destruct f as [f|f].
-      all: destruct He as [He|He] ; now try apply IHl with (n + 1)%nat.
-    + destruct He as [He|He].
-      - exists n. congruence.
-      - now apply IHl with (n + 1)%nat.
+  now rewrite !Zlength_correct, fields_to_cells__length.
 Qed.
 
-Lemma fields_to_cells__length (l: list FieldValue) (v: Addr) (n: nat):
-    length (fields_to_cells l v n) = length l.
+Lemma fields_to_cells__nth 
+  (n : nat) (l_raw : list FieldValue) 
+  (i : nat) (v : Addr) 
+  (e : Field) (Hn : 0 <= Z.of_nat n < Zlength l_raw) 
+  (He : nth n (fields_to_cells l_raw v i) Cell_inhabitant = inr e) : 
+  e = {| field_addr := v; field_index := n + i |}.
 Proof.
-    revert n ; induction l as [|f l IHl] ; intro n ; simpl ; try easy.
-    destruct f as [f|] ; try destruct f as [f|f] ; simpl.
-    all: now rewrite IHl.
-Qed.
-
-Lemma fields_to_cells__Zlength (l: list FieldValue) (v: Addr) (n: nat):
-    Zlength (fields_to_cells l v n) = Zlength l.
-Proof.
-    now rewrite !Zlength_correct, fields_to_cells__length.
-Qed.
-
-Lemma fields_to_cells__nth (n: nat) (l_raw: list FieldValue) (i: nat) (v: Addr) (e: Field)
-    (Hn: 0 <= Z.of_nat n < Zlength l_raw)
-    (He: nth n (fields_to_cells l_raw v i) Cell_inhabitant = inr e):
-    e = {| field_addr := v; field_index := n+i |}.
-Proof.
-  revert l_raw i v e Hn He ; induction n as [|n' IHn'] ; intros l_raw i v e Hn He.
-  - destruct l_raw as [| r l_raw]; try inversion He.
-    destruct r; [destruct s|]; simpl in He; now inversion He.
-  - destruct l_raw as [| r l_raw]; try inversion He.
+  (revert l_raw i v e Hn He; induction n as [| n' IHn']; intros l_raw i v e Hn He).
+  - (destruct l_raw as [| r l_raw]; try inversion He).
+    (destruct r; [ destruct s |  ]; simpl in He; now inversion He).
+  - (destruct l_raw as [| r l_raw]; try inversion He).
     replace (S n' + i)%nat with (n' + S i)%nat by lia.
     specialize (IHn' l_raw (S i) v e).
-    assert (0 <= Z.of_nat n' < Zlength l_raw) as Hn'.
+    (assert (Hn' : 0 <= Z.of_nat n' < Zlength l_raw)).
     {
-      rewrite Zlength_cons, Nat2Z.inj_succ in Hn.
+      (rewrite Zlength_cons, Nat2Z.inj_succ in Hn).
       lia.
     }
-    assert (nth n' (fields_to_cells l_raw v (S i)) Cell_inhabitant = inr e) as He'.
+    (assert (He' : nth n' (fields_to_cells l_raw v (S i)) Cell_inhabitant = inr e)).
     {
-        destruct r ; [destruct s|] ; simpl in He ; now replace (i + 1)%nat with (S i) in He by lia.
+      (destruct r; [ destruct s |  ]; simpl in He; now replace (i + 1)%nat with (S i) in He by lia).
     }
-    destruct r ; [destruct s|] ; simpl ; now apply IHn'.
+    (destruct r; [ destruct s |  ]; simpl; now apply IHn').
 Qed.
 
-Lemma fields_to_cells__n_doesnt_matter (i: nat) (l: list FieldValue) (v: Addr) (n m: nat) (gcptr: GC_Pointer)
-    (Hn: nth i (fields_to_cells l v n) Cell_inhabitant = inl (inr gcptr)):
-    nth i (fields_to_cells l v m) Cell_inhabitant = inl (inr gcptr).
+Lemma fields_to_cells__n_doesnt_matter 
+  (i : nat) (l : list FieldValue) 
+  (v : Addr) (n m : nat) 
+  (gcptr : GC_Pointer) 
+  (Hn : nth i (fields_to_cells l v n) Cell_inhabitant = inl (inr gcptr)) :
+  nth i (fields_to_cells l v m) Cell_inhabitant = inl (inr gcptr).
 Proof.
-    intros.
-    unfold fields_to_cells in *.
-    generalize dependent i.
-    generalize dependent n.
-    generalize dependent m.
-    induction l.
-    + intros; assumption.
-    + induction i.
-      - destruct a; [destruct s|]; simpl; intros; now try inversion Hn.
-      - destruct a; [destruct s|]; simpl; intro; now apply IHl with (m:=(m+1)%nat) in Hn.
+  (intros).
+  (unfold fields_to_cells in *).
+  generalize dependent i.
+  generalize dependent n.
+  generalize dependent m.
+  (induction l).
+  + (intros; assumption).
+  + (induction i).
+    - (destruct a; [ destruct s |  ]; simpl; intros; now try inversion Hn).
+    - (destruct a; [ destruct s |  ]; simpl; intro; now apply IHl with (m := (m + 1)%nat) in Hn).
 Qed.
 
-Lemma fields_to_cells__id (l: list FieldValue) (v: Addr) (n: Z) (gcptr: GC_Pointer)
-    (Hn: 0 <= n < Zlength l)
-    (Hgcptr: Znth n (fields_to_cells l v 0) = inl (inr gcptr)):
-    Znth n l = Some (inr gcptr).
+Lemma fields_to_cells__id 
+  (l : list FieldValue) 
+  (v : Addr) (n : Z) 
+  (gcptr : GC_Pointer) 
+  (Hn : 0 <= n < Zlength l) 
+  (Hgcptr : Znth n (fields_to_cells l v 0) = inl (inr gcptr)) : 
+  Znth n l = Some (inr gcptr).
 Proof.
-    rewrite <- nth_Znth; rewrite <- nth_Znth in Hgcptr; [| rewrite Zlength_correct in *..]; try rewrite fields_to_cells__length; [|assumption..].
-    generalize dependent n.
-    induction l.
-    - intros. rewrite nth_Znth in Hgcptr; try assumption.
-      unfold fields_to_cells in Hgcptr; rewrite Znth_nil in Hgcptr; inversion Hgcptr.
-    - intro n. induction (Z.to_nat n) eqn:?.
-      + intros. destruct a; [destruct s|]; simpl in *; try inversion Hgcptr; try reflexivity.
-      + intros. simpl in *. clear IHn0.
-        replace n0 with (Z.to_nat (Z.of_nat n0)) by apply Nat2Z.id.
-        assert (0 <= Z.of_nat n0 < Zlength l) as Hn0.
-        {
-          split; try lia.
-          apply Zsucc_lt_reg.
-          rewrite Zlength_cons in Hn.
-          rewrite <- Nat2Z.inj_succ, <- Heqn0, Z2Nat.id ; lia.
-        }
-        destruct a ; [destruct s|] ; simpl in Hgcptr ; apply IHl ; try easy.
-        all: apply fields_to_cells__n_doesnt_matter with (n:=1%nat) ; now rewrite Nat2Z.id.
+  (rewrite <- nth_Znth; rewrite <- nth_Znth in Hgcptr; [ idtac | rewrite Zlength_correct in *.. ];
+    try rewrite fields_to_cells__length; 
+    [ idtac | assumption.. ]).
+  generalize dependent n.
+  (induction l).
+  - (intros).
+    (rewrite nth_Znth in Hgcptr; try assumption).
+    (unfold fields_to_cells in Hgcptr; rewrite Znth_nil in Hgcptr; inversion Hgcptr).
+  - intro n.
+    (induction (Z.to_nat n) eqn:?).
+    + (intros).
+      (destruct a; [ destruct s |  ]; simpl in *; try inversion Hgcptr; try reflexivity).
+    + (intros).
+      (simpl in *).
+      clear IHn0.
+      replace n0 with (Z.to_nat (Z.of_nat n0)) by apply Nat2Z.id.
+      (assert (Hn0 : 0 <= Z.of_nat n0 < Zlength l)).
+      {
+        (split; try lia).
+        (apply Zsucc_lt_reg).
+        (rewrite Zlength_cons in Hn).
+        (rewrite <- Nat2Z.inj_succ, <- Heqn0, Z2Nat.id; lia).
+      }
+      (destruct a; [ destruct s |  ]; simpl in Hgcptr; apply IHl; try easy).
+      all: (apply fields_to_cells__n_doesnt_matter with (n := 1%nat); now rewrite Nat2Z.id).
 Qed.
 
+Definition heapgraph_block_cells 
+  (g : HeapGraph) (v : Addr) : 
+  list Cell := fields_to_cells (heapgraph_block g v).(block_fields) v O.
 
-Definition heapgraph_block_cells (g: HeapGraph) (v: Addr): list Cell :=
-  fields_to_cells (heapgraph_block g v).(block_fields) v O.
+Definition heapgraph_block_fields 
+  (g : HeapGraph) (v : Addr) : 
+  list Field := filter_sum_right (heapgraph_block_cells g v).
 
-Definition heapgraph_block_fields (g: HeapGraph) (v: Addr): list Field :=
-  filter_sum_right (heapgraph_block_cells g v).
+Definition heapgraph_block_is_no_scan 
+  (g : HeapGraph) (v : Addr) : Prop := 
+  NO_SCAN_TAG <= (heapgraph_block g v).(block_tag).
 
-
-Definition heapgraph_block_is_no_scan (g: HeapGraph) (v: Addr):
-    Prop
- := NO_SCAN_TAG <= (heapgraph_block g v).(block_tag)
-.
-
-
-Lemma heapgraph_block_is_no_scan__no_fields (g: HeapGraph) (v: Addr)
-    (Hv: heapgraph_block_is_no_scan g v):
-    heapgraph_block_fields g v = nil.
+Lemma heapgraph_block_is_no_scan__no_fields 
+  (g : HeapGraph) (v : Addr) 
+  (Hv : heapgraph_block_is_no_scan g v) : 
+  heapgraph_block_fields g v = nil.
 Proof.
-    apply block_tag__no_scan in Hv.
-    unfold heapgraph_block_fields.
-    destruct (filter_sum_right (heapgraph_block_cells g v)) as [|f ff] eqn:E ; try easy.
-    destruct Hv.
-    assert (In f (filter_sum_right (heapgraph_block_cells g v))) as Hf.
-    {
-      rewrite E.
-      now left.
-    }
-    rewrite <- filter_sum_right_In_iff in Hf.
-    clear ff E.
-    unfold heapgraph_block_cells in Hf.
-    remember (block_fields (heapgraph_block g v)) as xx eqn:Exx. clear Exx.
-    remember O as n eqn:En. clear En. revert n Hf.
-    induction xx as [|x xx IHxx] ; simpl ; intros n Hf ; try easy.
-    destruct x as [x|] ; try destruct x as [x|x] ; simpl in Hf ; try now left.
-    all: destruct Hf as [Hf|Hf] ; try easy.
-    all: right ; now apply IHxx with (n + 1)%nat.
+  (apply block_tag__no_scan in Hv).
+  (unfold heapgraph_block_fields).
+  (destruct (filter_sum_right (heapgraph_block_cells g v)) as [| f ff] eqn:E; try easy).
+  (destruct Hv).
+  (assert (Hf : In f (filter_sum_right (heapgraph_block_cells g v)))).
+  {
+    (rewrite E).
+    now left.
+  }
+  (rewrite <- filter_sum_right_In_iff in Hf).
+  clear ff E.
+  (unfold heapgraph_block_cells in Hf).
+  (remember (block_fields (heapgraph_block g v)) as xx eqn:Exx ).
+  clear Exx.
+  (remember O as n eqn:En ).
+  clear En.
+  revert n Hf.
+  (induction xx as [| x xx IHxx]; simpl; intros n Hf; try easy).
+  (destruct x as [x| ]; try destruct x as [x| x]; simpl in Hf; try now left).
+  all: (destruct Hf as [Hf| Hf]; try easy).
+  all: (right; now apply IHxx with (n + 1)%nat).
 Qed.
 
+Record heapgraph_has_block (g : HeapGraph) (v : Addr) : Prop :=
+ {
+  heapgraph_has_block__has_gen  : heapgraph_has_gen g (addr_gen v);
+  heapgraph_has_block__has_index  : heapgraph_generation_has_index g (addr_gen v) (addr_block v)
+ }.
 
-Record heapgraph_has_block (g: HeapGraph) (v: Addr): Prop
- := {
-    heapgraph_has_block__has_gen: heapgraph_has_gen g (addr_gen v);
-    heapgraph_has_block__has_index: heapgraph_generation_has_index g (addr_gen v) (addr_block v);
-}.
-Arguments heapgraph_has_block__has_gen [_] [_].
-Arguments heapgraph_has_block__has_index [_] [_].
+Arguments heapgraph_has_block__has_gen [_ _].
 
-Lemma heapgraph_generations_append__heapgraph_has_block (g : HeapGraph) (gi : Generation) (v : Addr)
-    (Hv: heapgraph_has_block g v):
-    heapgraph_has_block (heapgraph_generations_append g gi) v.
+Arguments heapgraph_has_block__has_index [_ _].
+
+Lemma heapgraph_generations_append__heapgraph_has_block 
+  (g : HeapGraph) (gi : Generation) 
+  (v : Addr) (Hv : heapgraph_has_block g v) : 
+  heapgraph_has_block (heapgraph_generations_append g gi) v.
 Proof.
-    destruct v as [gen idx]. destruct Hv; split; simpl in *.
-    - unfold heapgraph_has_gen in *. simpl. rewrite app_length. simpl. lia.
-    - unfold heapgraph_generation_has_index in *. rewrite heapgraph_generation__heapgraph_generations_append__old; assumption.
+  (destruct v as [gen idx]).
+  (destruct Hv; split; simpl in *).
+  - (unfold heapgraph_has_gen in *).
+    (simpl).
+    (rewrite app_length).
+    (simpl).
+    lia.
+  - (unfold heapgraph_generation_has_index in *).
+    (rewrite heapgraph_generation__heapgraph_generations_append__old; assumption).
 Qed.
 
-Lemma heapgraph_generations_append__heapgraph_has_block_inv (g : HeapGraph) (gi : Generation) (v : Addr)
-    (Hgi: generation_block_count gi = O)
-    (Hv: heapgraph_has_block (heapgraph_generations_append g gi) v):
-    heapgraph_has_block g v.
+Lemma heapgraph_generations_append__heapgraph_has_block_inv 
+  (g : HeapGraph) (gi : Generation) 
+  (v : Addr) (Hgi : generation_block_count gi = O) 
+  (Hv : heapgraph_has_block (heapgraph_generations_append g gi) v) : 
+  heapgraph_has_block g v.
 Proof.
-    pose proof (heapgraph_has_block__has_gen Hv) as Hgen.
-    pose proof (heapgraph_has_block__has_index Hv) as Hindex.
-    red in Hindex.
-    apply heapgraph_has_gen__heapgraph_generations_append in Hgen.
-    refine {|
-      heapgraph_has_block__has_gen := _;
-      heapgraph_has_block__has_index := _;
-    |}.
-    + destruct Hgen as [Hgen|Hgen] ; try easy.
-      rewrite Hgen, heapgraph_generation__heapgraph_generations_append__new in Hindex.
-      lia.
-    + destruct Hgen as [Hgen|Hgen].
-      - now rewrite heapgraph_generation__heapgraph_generations_append__old in Hindex.
-      - rewrite Hgen, heapgraph_generation__heapgraph_generations_append__new in Hindex.
-        lia.
-Qed.
-
-Lemma heapgraph_generations_append__heapgraph_block_ptr (g : HeapGraph) (gi : Generation) (v : Addr)
-    (Hv: heapgraph_has_block g v):
-    heapgraph_block_ptr (heapgraph_generations_append g gi) v = heapgraph_block_ptr g v.
-Proof.
-    unfold heapgraph_block_ptr. f_equal.
-    unfold heapgraph_generation_base.
-    destruct Hv.
-    rewrite if_true by (rewrite heapgraph_has_gen__heapgraph_generations_append ; now left).
-    rewrite if_true by easy.
-    now rewrite heapgraph_generation__heapgraph_generations_append__old.
-Qed.
-
-
-Definition heapgraph_generation_can_copy g from to:
-    Prop
- := generation_size from <= generation_size to - heapgraph_generation_size g to
-.
-
-Definition heapgraph_can_copy (g: HeapGraph):
-    Prop
- := forall n, heapgraph_has_gen g (S n) -> heapgraph_generation_can_copy g n (S n)
-.
-
-Definition heapgraph_can_copy_except (g: HeapGraph) (gen: nat):
-    Prop
- := forall n, n <> O -> n <> gen -> heapgraph_has_gen g n -> heapgraph_generation_can_copy g (pred n) n
-.
-
-Lemma heapgraph_can_copy_except__O (g: HeapGraph):
-    heapgraph_can_copy g <-> heapgraph_can_copy_except g O.
-Proof.
-    unfold heapgraph_can_copy, heapgraph_can_copy_except.
-    split.
-    + intros H n Hn _ Hgn.
-      destruct n as [|n] ; try easy.
-      now apply H.
-    + intros H n Hn.
-      specialize (H (S n)).
-      now apply H.
-Qed.
-
-Lemma heapgraph_can_copy__complete (g: HeapGraph) (i: nat)
-    (Hg: heapgraph_can_copy_except g (S i))
-    (Hi: heapgraph_generation_can_copy g i (S i)):
-    heapgraph_can_copy g.
-Proof.
-    unfold heapgraph_can_copy_except in Hg.
-    unfold heapgraph_can_copy in *.
-    intros n Hn.
-    destruct (Nat.eq_dec n i) as [E|Hn__i].
-    + now subst.
-    + specialize (Hg (S n)).
-      apply Hg ; now try congruence.
-Qed.
-
-
-Record heapgraph_has_field (g: HeapGraph) (e: Field):
-    Prop
- := {
-    heapgraph_has_field__has_block: heapgraph_has_block g (field_addr e);
-    heapgraph_has_field__in: In e (heapgraph_block_fields g (field_addr e));
-}.
-Arguments heapgraph_has_field__has_block [_] [_].
-Arguments heapgraph_has_field__in [_] [_].
-
-Definition gen2gen_no_edge (g: HeapGraph) (gen1 gen2: nat):
-    Prop
- := forall vidx eidx,
-    let e := {| field_addr := {| addr_gen := gen1; addr_block := vidx |}; field_index := eidx |}
- in heapgraph_has_field g e -> addr_gen (dst g e) <> gen2.
-
-Definition no_edge2gen (g: HeapGraph) (gen: nat):
-    Prop
- := forall another, another <> gen -> gen2gen_no_edge g another gen.
-
-Definition no_backward_edge (g: HeapGraph):
-    Prop
- := forall gen1 gen2, (gen1 > gen2)%nat -> gen2gen_no_edge g gen1 gen2
-.
-
-Definition graph_gen_clear (g: HeapGraph) (gen: nat):
-    Prop
- := generation_block_count (heapgraph_generation g gen) = O
-.
-
-
-Definition firstn_gen_clear (g: HeapGraph) (n: nat): Prop :=
-  forall i, (i < n)%nat -> graph_gen_clear g i.
-
-Lemma fgc_nbe_no_edge2gen (g : HeapGraph) (n : nat)
-    (Hn: firstn_gen_clear g n)
-    (Hg: no_backward_edge g):
-    no_edge2gen g n.
-Proof.
-    intros m Hm.
-    destruct (lt_eq_lt_dec m n) as [[Hmn|Hmn]|Hmn] ; try easy.
-    + intros vidx eidx f Hf En. subst f.
-      pose proof (heapgraph_has_block__has_index (heapgraph_has_field__has_block Hf)) as F.
-      specialize (Hn _ Hmn).
-      red in Hn, F. simpl in F.
-      rewrite Hn in F.
-      lia.
-    + apply Hg.
+  (pose proof (heapgraph_has_block__has_gen Hv) as Hgen).
+  (pose proof (heapgraph_has_block__has_index Hv) as Hindex).
+  (red in Hindex).
+  (apply heapgraph_has_gen__heapgraph_generations_append in Hgen).
+  refine {| heapgraph_has_block__has_gen := _; heapgraph_has_block__has_index := _ |}.
+  + (destruct Hgen as [Hgen| Hgen]; try easy).
+    (rewrite Hgen, heapgraph_generation__heapgraph_generations_append__new in Hindex).
+    lia.
+  + (destruct Hgen as [Hgen| Hgen]).
+    - now rewrite heapgraph_generation__heapgraph_generations_append__old in Hindex.
+    - (rewrite Hgen, heapgraph_generation__heapgraph_generations_append__new in Hindex).
       lia.
 Qed.
 
-Lemma firstn_gen_clear_add: forall g gi i,
-    heapgraph_has_gen g (Z.to_nat i) -> firstn_gen_clear g (Z.to_nat i) ->
-    firstn_gen_clear (heapgraph_generations_append g gi) (Z.to_nat i).
+Lemma heapgraph_generations_append__heapgraph_block_ptr 
+  (g : HeapGraph) (gi : Generation) 
+  (v : Addr) (Hv : heapgraph_has_block g v) :
+  heapgraph_block_ptr (heapgraph_generations_append g gi) v = heapgraph_block_ptr g v.
 Proof.
-  intros. unfold firstn_gen_clear, graph_gen_clear in *. intros. specialize (H0 _ H1).
-  rewrite heapgraph_generation__heapgraph_generations_append__old; auto. unfold heapgraph_has_gen in *. lia.
+  (unfold heapgraph_block_ptr).
+  f_equal.
+  (unfold heapgraph_generation_base).
+  (destruct Hv).
+  (rewrite if_true by (rewrite heapgraph_has_gen__heapgraph_generations_append; now left)).
+  (rewrite if_true by easy).
+  now rewrite heapgraph_generation__heapgraph_generations_append__old.
 Qed.
 
+Definition heapgraph_generation_can_copy 
+  g from to : Prop := 
+  generation_size from <= generation_size to - heapgraph_generation_size g to.
 
-Definition egeneration (e: Field): nat := addr_gen (field_addr e).
+Definition heapgraph_can_copy 
+  (g : HeapGraph) : Prop := 
+  forall n, heapgraph_has_gen g (S n) -> heapgraph_generation_can_copy g n (S n).
 
+Definition heapgraph_can_copy_except 
+  (g : HeapGraph) (gen : nat) : Prop :=
+  forall n, n <> O -> n <> gen -> heapgraph_has_gen g n -> heapgraph_generation_can_copy g (pred n) n.
 
-Definition no_dangling_dst (g: HeapGraph): Prop :=
-  forall v, heapgraph_has_block g v ->
-            forall e, In e (heapgraph_block_fields g v) -> heapgraph_has_block g (dst g e).
-
-Lemma heapgraph_block_fields_In: forall g v s,
-    In {| field_addr := v; field_index := s|} (heapgraph_block_fields g v) <-> In s (map field_index (heapgraph_block_fields g v)).
+Lemma heapgraph_can_copy_except__O (g : HeapGraph) : heapgraph_can_copy g <-> heapgraph_can_copy_except g O.
 Proof.
-  intros. unfold heapgraph_block_fields, heapgraph_block_cells. remember (block_fields (heapgraph_block g v)).
-  remember O as n. clear Heqn Heql. revert n. induction l; intros; simpl ; try easy.
-  destruct a as [a|] ; try destruct a as [a|a] ; simpl.
-  all: rewrite IHl ; try easy.
-  intuition. inversion H0. left; reflexivity.
+  (unfold heapgraph_can_copy, heapgraph_can_copy_except).
+  split.
+  + (intros H n Hn _ Hgn).
+    (destruct n as [| n]; try easy).
+    now apply H.
+  + (intros H n Hn).
+    specialize (H (S n)).
+    now apply H.
 Qed.
 
-Lemma heapgraph_block_fields_fst: forall g v e, In e (heapgraph_block_fields g v) -> field_addr e = v.
+Lemma heapgraph_can_copy__complete 
+  (g : HeapGraph) (i : nat) 
+  (Hg : heapgraph_can_copy_except g (S i)) 
+  (Hi : heapgraph_generation_can_copy g i (S i)) : 
+  heapgraph_can_copy g.
 Proof.
-  intros g v e. unfold heapgraph_block_fields, heapgraph_block_cells. remember (block_fields (heapgraph_block g v)).
-  remember O as n. clear Heqn Heql. revert n. induction l; intros; simpl in *.
-  - exfalso; assumption.
-  - destruct a; [destruct s|]; simpl in *;
-      [| | destruct H; [subst e; simpl; reflexivity|]]; apply IHl in H; assumption.
+  (unfold heapgraph_can_copy_except in Hg).
+  (unfold heapgraph_can_copy in *).
+  (intros n Hn).
+  (destruct (Nat.eq_dec n i) as [E| Hn__i]).
+  + now subst.
+  + specialize (Hg (S n)).
+    (apply Hg; now try congruence).
 Qed.
 
+Record heapgraph_has_field (g : HeapGraph) (e : Field) : Prop :=
+ {
+  heapgraph_has_field__has_block  : heapgraph_has_block g (field_addr e);
+  heapgraph_has_field__in  : In e (heapgraph_block_fields g (field_addr e))
+ }.
 
-Definition v_in_range (v: val) (start: val) (n: Z): Prop :=
-  exists i, 0 <= i < n /\ v = offset_val i start.
+Arguments heapgraph_has_field__has_block [_ _].
 
+Arguments heapgraph_has_field__in [_ _].
 
-Lemma heapgraph_block_cells_eq_length: forall g v,
-    Zlength (heapgraph_block_cells g v) = Zlength (block_fields (heapgraph_block g v)).
+Definition gen2gen_no_edge 
+  (g : HeapGraph) (gen1 gen2 : nat) : Prop :=
+  forall vidx eidx,
+  let e := {| field_addr := {| addr_gen := gen1; addr_block := vidx |}; field_index := eidx |} in
+  heapgraph_has_field g e -> addr_gen (dst g e) <> gen2.
+
+Definition no_edge2gen 
+  (g : HeapGraph) (gen : nat) : Prop := 
+  forall another, another <> gen -> gen2gen_no_edge g another gen.
+
+Definition no_backward_edge 
+  (g : HeapGraph) : Prop := 
+  forall gen1 gen2, (gen1 > gen2)%nat -> gen2gen_no_edge g gen1 gen2.
+
+Definition graph_gen_clear 
+  (g : HeapGraph) (gen : nat) : Prop := 
+  generation_block_count (heapgraph_generation g gen) = O.
+
+Definition firstn_gen_clear (g : HeapGraph) (n : nat) : Prop := forall i, (i < n)%nat -> graph_gen_clear g i.
+
+Lemma fgc_nbe_no_edge2gen 
+  (g : HeapGraph) (n : nat) 
+  (Hn : firstn_gen_clear g n) 
+  (Hg : no_backward_edge g) : 
+  no_edge2gen g n.
 Proof.
-  unfold heapgraph_block_cells. intros.
-  rewrite !Zlength_correct, fields_to_cells__length. reflexivity.
+  (intros m Hm).
+  (destruct (lt_eq_lt_dec m n) as [[Hmn| Hmn]| Hmn]; try easy).
+  + (intros vidx eidx f Hf En).
+    subst f.
+    (pose proof (heapgraph_has_block__has_index (heapgraph_has_field__has_block Hf)) as F).
+    specialize (Hn _ Hmn).
+    (red in Hn, F).
+    (simpl in F).
+    (rewrite Hn in F).
+    lia.
+  + (apply Hg).
+    lia.
 Qed.
 
-Lemma heapgraph_block_cells_Znth_edge: forall g v n e,
-    0 <= n < Zlength (block_fields (heapgraph_block g v)) ->
-    Znth n (heapgraph_block_cells g v) = inr e -> e = {| field_addr := v; field_index := Z.to_nat n |}.
+Lemma firstn_gen_clear_add :
+  forall g gi i,
+  heapgraph_has_gen g (Z.to_nat i) ->
+  firstn_gen_clear g (Z.to_nat i) -> firstn_gen_clear (heapgraph_generations_append g gi) (Z.to_nat i).
 Proof.
-  intros. rewrite <- nth_Znth in H0. 2: rewrite heapgraph_block_cells_eq_length; assumption.
-  apply fields_to_cells__nth in H0.
+  (intros).
+  (unfold firstn_gen_clear, graph_gen_clear in *).
+  (intros).
+  specialize (H0 _ H1).
+  (rewrite heapgraph_generation__heapgraph_generations_append__old; auto).
+  (unfold heapgraph_has_gen in *).
+  lia.
+Qed.
+
+Definition egeneration (e : Field) : nat := addr_gen (field_addr e).
+
+Definition no_dangling_dst 
+  (g : HeapGraph) : Prop :=
+  forall v, heapgraph_has_block g v -> forall e, In e (heapgraph_block_fields g v) -> heapgraph_has_block g (dst g e).
+
+Lemma heapgraph_block_fields_In :
+  forall g v s,
+  In {| field_addr := v; field_index := s |} (heapgraph_block_fields g v) <->
+  In s (map field_index (heapgraph_block_fields g v)).
+Proof.
+  (intros).
+  (unfold heapgraph_block_fields, heapgraph_block_cells).
+  (remember (block_fields (heapgraph_block g v))).
+  (remember O as n).
+  clear Heqn Heql.
+  revert n.
+  (induction l; intros; simpl; try easy).
+  (destruct a as [a| ]; try destruct a as [a| a]; simpl).
+  all: (rewrite IHl; try easy).
+  intuition.
+  (inversion H0).
+  (left; reflexivity).
+Qed.
+
+Lemma heapgraph_block_fields_fst : forall g v e, In e (heapgraph_block_fields g v) -> field_addr e = v.
+Proof.
+  (intros g v e).
+  (unfold heapgraph_block_fields, heapgraph_block_cells).
+  (remember (block_fields (heapgraph_block g v))).
+  (remember O as n).
+  clear Heqn Heql.
+  revert n.
+  (induction l; intros; simpl in *).
+  - (exfalso; assumption).
+  - (destruct a; [ destruct s |  ]; simpl in *; [  |  | destruct H; [ subst e; simpl; reflexivity |  ] ];
+      apply IHl in H; assumption).
+Qed.
+
+Definition v_in_range (v : val) (start : val) (n : Z) : Prop := exists i, 0 <= i < n /\ v = offset_val i start.
+
+Lemma heapgraph_block_cells_eq_length :
+  forall g v, Zlength (heapgraph_block_cells g v) = Zlength (block_fields (heapgraph_block g v)).
+Proof.
+  (unfold heapgraph_block_cells).
+  (intros).
+  (rewrite !Zlength_correct, fields_to_cells__length).
+  reflexivity.
+Qed.
+
+Lemma heapgraph_block_cells_Znth_edge :
+  forall g v n e,
+  0 <= n < Zlength (block_fields (heapgraph_block g v)) ->
+  Znth n (heapgraph_block_cells g v) = inr e -> e = {| field_addr := v; field_index := Z.to_nat n |}.
+Proof.
+  (intros).
+  (rewrite <- nth_Znth in H0).
+  2: (rewrite heapgraph_block_cells_eq_length; assumption).
+  (apply fields_to_cells__nth in H0).
   - now rewrite Nat.add_0_r in H0.
   - now rewrite Z2Nat.id.
 Qed.
 
-Lemma heapgraph_block_cells_edge_unique: forall g e v1 v2 n m,
-    0 <= n < Zlength (heapgraph_block_cells g v1) ->
-    0 <= m < Zlength (heapgraph_block_cells g v2) ->
-    Znth n (heapgraph_block_cells g v1) = inr e ->
-    Znth m (heapgraph_block_cells g v2) = inr e ->
-    n = m /\ v1 = v2.
+Lemma heapgraph_block_cells_edge_unique :
+  forall g e v1 v2 n m,
+  0 <= n < Zlength (heapgraph_block_cells g v1) ->
+  0 <= m < Zlength (heapgraph_block_cells g v2) ->
+  Znth n (heapgraph_block_cells g v1) = inr e -> Znth m (heapgraph_block_cells g v2) = inr e -> n = m /\ v1 = v2.
 Proof.
-  intros. unfold heapgraph_block_cells in *.
-  rewrite fields_to_cells__Zlength in *.
-  assert (0 <= Z.of_nat (Z.to_nat n) < Zlength (block_fields (heapgraph_block g v1))) by
-      (destruct H; split; rewrite Z2Nat.id; assumption).
-  rewrite <- nth_Znth in H1 by
-      (rewrite fields_to_cells__Zlength; assumption).
-  assert (0 <= Z.of_nat (Z.to_nat m) < Zlength (block_fields (heapgraph_block g v2))) by
-       (destruct H0; split; rewrite Z2Nat.id; assumption).
-  rewrite <- nth_Znth in H2 by
-      (rewrite fields_to_cells__Zlength; assumption).
-  pose proof (fields_to_cells__nth
-                (Z.to_nat n) (block_fields (heapgraph_block g v1)) 0 v1 e H3 H1).
-  pose proof (fields_to_cells__nth
-                (Z.to_nat m) (block_fields (heapgraph_block g v2)) 0 v2 e H4 H2).
-  rewrite H5 in H6. inversion H6.
-  rewrite Nat.add_cancel_r, Z2Nat.inj_iff in H9 by lia.
-  split; [assumption | reflexivity].
+  (intros).
+  (unfold heapgraph_block_cells in *).
+  (rewrite fields_to_cells__Zlength in *).
+  (assert (0 <= Z.of_nat (Z.to_nat n) < Zlength (block_fields (heapgraph_block g v1))) by
+    (destruct H; split; rewrite Z2Nat.id; assumption)).
+  (rewrite <- nth_Znth in H1 by (rewrite fields_to_cells__Zlength; assumption)).
+  (assert (0 <= Z.of_nat (Z.to_nat m) < Zlength (block_fields (heapgraph_block g v2))) by
+    (destruct H0; split; rewrite Z2Nat.id; assumption)).
+  (rewrite <- nth_Znth in H2 by (rewrite fields_to_cells__Zlength; assumption)).
+  (pose proof (fields_to_cells__nth (Z.to_nat n) (block_fields (heapgraph_block g v1)) 0 v1 e H3 H1)).
+  (pose proof (fields_to_cells__nth (Z.to_nat m) (block_fields (heapgraph_block g v2)) 0 v2 e H4 H2)).
+  (rewrite H5 in H6).
+  (inversion H6).
+  (rewrite Nat.add_cancel_r, Z2Nat.inj_iff in H9 by lia).
+  (split; [ assumption | reflexivity ]).
 Qed.
 
+Definition heapgraph_block_cells_vals 
+  (g : HeapGraph) (v : Addr) : 
+  list val :=
+  let vb := heapgraph_block g v in
+  let original_fields_val := map (heapgraph_cell_val g) (heapgraph_block_cells g v) in
+  if vb.(block_mark)
+  then heapgraph_block_ptr g vb.(block_copied_vertex) :: tl original_fields_val
+  else original_fields_val.
 
-Definition heapgraph_block_cells_vals (g: HeapGraph) (v: Addr):
-    list val
- := let vb := heapgraph_block g v
- in let original_fields_val := map (heapgraph_cell_val g) (heapgraph_block_cells g v)
- in if vb.(block_mark)
-    then heapgraph_block_ptr g vb.(block_copied_vertex) :: tl original_fields_val
-    else original_fields_val.
-
-Lemma fields_eq_length: forall g v,
-    Zlength (heapgraph_block_cells_vals g v) = Zlength (block_fields (heapgraph_block g v)).
+Lemma fields_eq_length :
+  forall g v, Zlength (heapgraph_block_cells_vals g v) = Zlength (block_fields (heapgraph_block g v)).
 Proof.
-  intros. rewrite !Zlength_correct. f_equal. unfold heapgraph_block_cells_vals, heapgraph_block_cells.
-  destruct (block_mark (heapgraph_block g v)).
-  - destruct (block_fields_head__cons (heapgraph_block g v)) as [r [l [? ?]]].
-    rewrite H; simpl; destruct r; [destruct s|]; simpl;
-      rewrite map_length, fields_to_cells__length; reflexivity.
-  - rewrite map_length, fields_to_cells__length. reflexivity.
+  (intros).
+  (rewrite !Zlength_correct).
+  f_equal.
+  (unfold heapgraph_block_cells_vals, heapgraph_block_cells).
+  (destruct (block_mark (heapgraph_block g v))).
+  - (destruct (block_fields_head__cons (heapgraph_block g v)) as [r [l [? ?]]]).
+    (rewrite H; simpl; destruct r; [ destruct s |  ]; simpl; rewrite map_length, fields_to_cells__length; reflexivity).
+  - (rewrite map_length, fields_to_cells__length).
+    reflexivity.
 Qed.
 
-Lemma mfv_unmarked_all_is_ptr_or_int: forall (g : HeapGraph) (v : Addr),
-    no_dangling_dst g -> heapgraph_has_block g v ->
-    Forall is_pointer_or_integer (map (heapgraph_cell_val g) (heapgraph_block_cells g v)).
+Lemma mfv_unmarked_all_is_ptr_or_int :
+  forall (g : HeapGraph) (v : Addr),
+  no_dangling_dst g ->
+  heapgraph_has_block g v -> Forall is_pointer_or_integer (map (heapgraph_cell_val g) (heapgraph_block_cells g v)).
 Proof.
-  intros. rewrite Forall_forall. intros f ?. apply list_in_map_inv in H1.
-  destruct H1 as [x [? ?]]. destruct x as [[? | ?] | ?]; simpl in H1; subst.
-  - unfold odd_Z2val. exact I.
-  - destruct g0. exact I.
-  - apply isptr_is_pointer_or_integer. unfold heapgraph_block_ptr.
-    rewrite isptr_offset_val. apply heapgraph_generation_base__isptr.
-    apply filter_sum_right_In_iff, H in H2; [destruct H2|]; assumption.
+  (intros).
+  (rewrite Forall_forall).
+  (intros f ?).
+  (apply list_in_map_inv in H1).
+  (destruct H1 as [x [? ?]]).
+  (destruct x as [[?| ?]| ?]; simpl in H1; subst).
+  - (unfold odd_Z2val).
+    exact I.
+  - (destruct g0).
+    exact I.
+  - (apply isptr_is_pointer_or_integer).
+    (unfold heapgraph_block_ptr).
+    (rewrite isptr_offset_val).
+    (apply heapgraph_generation_base__isptr).
+    (apply filter_sum_right_In_iff, H in H2; [ destruct H2 |  ]; assumption).
 Qed.
 
-Definition copy_compatible (g: HeapGraph): Prop :=
-  forall v, heapgraph_has_block g v -> (heapgraph_block g v).(block_mark) = true ->
-            heapgraph_has_block g (heapgraph_block g v).(block_copied_vertex) /\
-            addr_gen v <> addr_gen (heapgraph_block g v).(block_copied_vertex).
+Definition copy_compatible 
+  (g : HeapGraph) : Prop :=
+  forall v,
+  heapgraph_has_block g v ->
+  (heapgraph_block g v).(block_mark) = true ->
+  heapgraph_has_block g (heapgraph_block g v).(block_copied_vertex) /\
+  addr_gen v <> addr_gen (heapgraph_block g v).(block_copied_vertex).
 
-Lemma lgd_copy_compatible (g: HeapGraph) (v': Addr) (e: Field)
-    (Hg: copy_compatible g):
-    copy_compatible (labeledgraph_gen_dst g e v').
+Lemma lgd_copy_compatible 
+  (g : HeapGraph) (v' : Addr) 
+  (e : Field) (Hg : copy_compatible g) : 
+  copy_compatible (labeledgraph_gen_dst g e v').
 Proof.
-    unfold copy_compatible in *.
-    intros v Jv E.
-    intuition.
-    + refine {|
-        heapgraph_has_block__has_gen := _;
-        heapgraph_has_block__has_index := _;
-      |} ; intuition.
-      - admit.
-      - admit.
-    + admit.
+  (unfold copy_compatible in *).
+  (intros v Jv E).
+  intuition.
+  + (refine {| heapgraph_has_block__has_gen := _; heapgraph_has_block__has_index := _ |}; intuition).
+    - admit.
+    - admit.
+  + admit.
 Admitted.
 
+Definition heapgraph_generation_is_unmarked 
+  (g : HeapGraph) (gen : nat) : Prop :=
+  heapgraph_has_gen g gen ->
+  forall idx,
+  heapgraph_generation_has_index g gen idx ->
+  (heapgraph_block g {| addr_gen := gen; addr_block := idx |}).(block_mark) = false.
 
-Definition heapgraph_generation_is_unmarked (g: HeapGraph) (gen: nat):
-    Prop
- := heapgraph_has_gen g gen ->
-    forall idx,
-    heapgraph_generation_has_index g gen idx ->
-    (heapgraph_block g {| addr_gen := gen; addr_block := idx |}).(block_mark) = false
-.
+Definition graph_unmarked 
+  (g : HeapGraph) : Prop := 
+  forall v, heapgraph_has_block g v -> block_mark (heapgraph_block g v) = false.
 
-
-Definition graph_unmarked (g: HeapGraph): Prop := forall v,
-    heapgraph_has_block g v -> block_mark (heapgraph_block g v) = false.
-
-Lemma graph_heapgraph_generation_is_unmarked_iff (g: HeapGraph):
-    graph_unmarked g <-> forall gen, heapgraph_generation_is_unmarked g gen.
+Lemma graph_heapgraph_generation_is_unmarked_iff 
+  (g : HeapGraph) : graph_unmarked g <-> (forall gen, heapgraph_generation_is_unmarked g gen).
 Proof.
-    unfold graph_unmarked, heapgraph_generation_is_unmarked.
-    split; intros.
-    + apply H.
-      now refine {|
-        heapgraph_has_block__has_gen := _ ;
-        heapgraph_has_block__has_index := _;
-      |}.
-    + pose proof (heapgraph_has_block__has_gen H0) as Hgen.
-      pose proof (heapgraph_has_block__has_index H0) as Hindex.
-      destruct v as [gen idx].
-      now apply H.
+  (unfold graph_unmarked, heapgraph_generation_is_unmarked).
+  (split; intros).
+  + (apply H).
+    now refine {| heapgraph_has_block__has_gen := _; heapgraph_has_block__has_index := _ |}.
+  + (pose proof (heapgraph_has_block__has_gen H0) as Hgen).
+    (pose proof (heapgraph_has_block__has_index H0) as Hindex).
+    (destruct v as [gen idx]).
+    now apply H.
 Qed.
 
-Lemma graph_unmarked_copy_compatible: forall g,
-    graph_unmarked g -> copy_compatible g.
+Lemma graph_unmarked_copy_compatible : forall g, graph_unmarked g -> copy_compatible g.
 Proof.
-  intros. red in H |-* . intros. apply H in H0. rewrite H0 in H1. inversion H1.
+  (intros).
+  (red in H |- *).
+  (intros).
+  (apply H in H0).
+  (rewrite H0 in H1).
+  (inversion H1).
 Qed.
 
-
-Lemma mfv_all_is_ptr_or_int: forall g v,
-    copy_compatible g -> no_dangling_dst g -> heapgraph_has_block g v ->
-    Forall is_pointer_or_integer (heapgraph_block_cells_vals g v).
+Lemma mfv_all_is_ptr_or_int :
+  forall g v,
+  copy_compatible g ->
+  no_dangling_dst g -> heapgraph_has_block g v -> Forall is_pointer_or_integer (heapgraph_block_cells_vals g v).
 Proof.
-  intros. rewrite Forall_forall. intros f ?. unfold heapgraph_block_cells_vals in H2.
-  pose proof (mfv_unmarked_all_is_ptr_or_int _ _ H0 H1). rewrite Forall_forall in H3.
-  specialize (H3 f). destruct (block_mark (heapgraph_block g v)) eqn:? . 2: apply H3; assumption.
-  simpl in H2. destruct H2. 2: apply H3, In_tail; assumption.
-  subst f. unfold heapgraph_block_ptr. apply isptr_is_pointer_or_integer.
-  rewrite isptr_offset_val. apply heapgraph_generation_base__isptr, (proj1 (H _ H1 Heqb)).
+  (intros).
+  (rewrite Forall_forall).
+  (intros f ?).
+  (unfold heapgraph_block_cells_vals in H2).
+  (pose proof (mfv_unmarked_all_is_ptr_or_int _ _ H0 H1)).
+  (rewrite Forall_forall in H3).
+  specialize (H3 f).
+  (destruct (block_mark (heapgraph_block g v)) eqn:?).
+  2: (apply H3; assumption).
+  (simpl in H2).
+  (destruct H2).
+  2: (apply H3, In_tail; assumption).
+  subst f.
+  (unfold heapgraph_block_ptr).
+  (apply isptr_is_pointer_or_integer).
+  (rewrite isptr_offset_val).
+  (apply heapgraph_generation_base__isptr, (proj1 (H _ H1 Heqb))).
 Qed.
 
-
-
-Lemma heapgraph_block_cells_the_same: forall (g1 g2: HeapGraph) v,
-    (forall e, dst g1 e = dst g2 e) ->
-    (forall v, heapgraph_block g1 v = heapgraph_block g2 v) ->
-    map generation_base (heapgraph_generations g1).(generations) = map generation_base (heapgraph_generations g2).(generations) ->
-    heapgraph_block_cells_vals g1 v = heapgraph_block_cells_vals g2 v.
+Lemma heapgraph_block_cells_the_same :
+  forall (g1 g2 : HeapGraph) v,
+  (forall e, dst g1 e = dst g2 e) ->
+  (forall v, heapgraph_block g1 v = heapgraph_block g2 v) ->
+  map generation_base (heapgraph_generations g1).(generations) =
+  map generation_base (heapgraph_generations g2).(generations) ->
+  heapgraph_block_cells_vals g1 v = heapgraph_block_cells_vals g2 v.
 Proof.
-  intros. unfold heapgraph_block_cells_vals, heapgraph_block_cells. remember O. clear Heqn. rewrite H0.
-  remember (block_fields (heapgraph_block g2 v)) as l. clear Heql.
-  cut (forall fl, map (heapgraph_cell_val g1) fl = map (heapgraph_cell_val g2) fl).
-  - intros. rewrite H2. rewrite (heapgraph_block_ptr__eq g1 g2) by assumption.
+  (intros).
+  (unfold heapgraph_block_cells_vals, heapgraph_block_cells).
+  (remember O).
+  clear Heqn.
+  (rewrite H0).
+  (remember (block_fields (heapgraph_block g2 v)) as l).
+  clear Heql.
+  (cut (forall fl, map (heapgraph_cell_val g1) fl = map (heapgraph_cell_val g2) fl)).
+  - (intros).
+    (rewrite H2).
+    (rewrite (heapgraph_block_ptr__eq g1 g2) by assumption).
     reflexivity.
-  - apply map_ext. intros. unfold heapgraph_cell_val. destruct a. 1: reflexivity.
-    rewrite H. apply heapgraph_block_ptr__eq; assumption.
+  - (apply map_ext).
+    (intros).
+    (unfold heapgraph_cell_val).
+    (destruct a).
+    1: reflexivity.
+    (rewrite H).
+    (apply heapgraph_block_ptr__eq; assumption).
 Qed.
 
-
-Definition unmarked_gen_size (g: HeapGraph) (gen: nat) :=
+Definition unmarked_gen_size 
+  (g : HeapGraph) (gen : nat) :=
   fold_left (heapgraph_block_size_accum g gen)
-            (filter (fun i => negb (heapgraph_block g {| addr_gen := gen; addr_block := i |}).(block_mark))
-                    (nat_inc_list (generation_block_count (heapgraph_generation g gen)))) 0.
+    (filter (fun i => negb (heapgraph_block g {| addr_gen := gen; addr_block := i |}).(block_mark))
+       (nat_inc_list (generation_block_count (heapgraph_generation g gen)))) 0.
 
-Lemma unmarked_gen_size_le: forall g n, unmarked_gen_size g n <= heapgraph_generation_size g n.
+Lemma unmarked_gen_size_le : forall g n, unmarked_gen_size g n <= heapgraph_generation_size g n.
 Proof.
-  intros g gen. unfold unmarked_gen_size, heapgraph_generation_size, heapgraph_block_size_prev.
-  apply fold_left_mono_filter;
-    [intros; rewrite Z.le_lteq; left; apply heapgraph_block_size_accum__mono | apply heapgraph_block_size_accum__comm].
+  (intros g gen).
+  (unfold unmarked_gen_size, heapgraph_generation_size, heapgraph_block_size_prev).
+  (apply fold_left_mono_filter;
+    [ intros; rewrite Z.le_lteq; left; apply heapgraph_block_size_accum__mono
+    | apply heapgraph_block_size_accum__comm ]).
 Qed.
 
-Lemma single_unmarked_le: forall g v,
-    heapgraph_has_block g v -> block_mark (heapgraph_block g v) = false ->
-    heapgraph_block_size g v <= unmarked_gen_size g (addr_gen v).
+Lemma single_unmarked_le :
+  forall g v,
+  heapgraph_has_block g v ->
+  block_mark (heapgraph_block g v) = false -> heapgraph_block_size g v <= unmarked_gen_size g (addr_gen v).
 Proof.
-  intros. unfold unmarked_gen_size.
-  remember (filter (fun i : nat => negb (block_mark (heapgraph_block g {| addr_gen := addr_gen v; addr_block := i |})))
-                   (nat_inc_list (generation_block_count (heapgraph_generation g (addr_gen v))))).
-  assert (In (addr_block v) l). {
-    subst l. rewrite filter_In. split.
-    - rewrite nat_inc_list_In_iff.
+  (intros).
+  (unfold unmarked_gen_size).
+  (remember
+    (filter (fun i : nat => negb (block_mark (heapgraph_block g {| addr_gen := addr_gen v; addr_block := i |})))
+       (nat_inc_list (generation_block_count (heapgraph_generation g (addr_gen v)))))).
+  (assert (In (addr_block v) l)).
+  {
+    subst l.
+    (rewrite filter_In).
+    split.
+    - (rewrite nat_inc_list_In_iff).
       now apply heapgraph_has_block__has_index.
-    - destruct v; simpl. rewrite negb_true_iff. apply H0. }
-  apply In_Permutation_cons in H1. destruct H1 as [l1 ?]. symmetry in H1.
-  change (addr_block v :: l1) with ([addr_block v] ++ l1) in H1.
-  transitivity (fold_left (heapgraph_block_size_accum g (addr_gen v)) [addr_block v] 0).
-  - simpl. destruct v; simpl. apply Z.le_refl.
-  - apply (fold_left_Z_mono (heapgraph_block_size_accum g (addr_gen v)) [addr_block v] l1 l 0);
-      [intros; apply Z.le_lteq; left; apply heapgraph_block_size_accum__mono | apply heapgraph_block_size_accum__comm | apply H1].
+    - (destruct v; simpl).
+      (rewrite negb_true_iff).
+      (apply H0).
+  }
+  (apply In_Permutation_cons in H1).
+  (destruct H1 as [l1 ?]).
+  symmetry in H1.
+  (change (addr_block v :: l1) with ([addr_block v] ++ l1) in H1).
+  (transitivity (fold_left (heapgraph_block_size_accum g (addr_gen v)) [addr_block v] 0)).
+  - (simpl).
+    (destruct v; simpl).
+    (apply Z.le_refl).
+  - (apply (fold_left_Z_mono (heapgraph_block_size_accum g (addr_gen v)) [addr_block v] l1 l 0);
+      [ intros; apply Z.le_lteq; left; apply heapgraph_block_size_accum__mono
+      | apply heapgraph_block_size_accum__comm
+      | apply H1 ]).
 Qed.
 
-
-Lemma heapgraph_block_header__heapgraph_generations_append: forall g gi v,
-    heapgraph_block_header g v = heapgraph_block_header (heapgraph_generations_append g gi) v.
-Proof. intros. unfold heapgraph_block_header. reflexivity. Qed.
-
-Lemma ang_heapgraph_block_cells_vals_old: forall g gi v,
-    heapgraph_has_block g v -> copy_compatible g -> no_dangling_dst g ->
-    heapgraph_block_cells_vals g v = heapgraph_block_cells_vals (heapgraph_generations_append g gi) v.
+Lemma heapgraph_block_header__heapgraph_generations_append :
+  forall g gi v, heapgraph_block_header g v = heapgraph_block_header (heapgraph_generations_append g gi) v.
 Proof.
-  intros. unfold heapgraph_block_cells_vals. simpl.
-  assert (map (heapgraph_cell_val g) (heapgraph_block_cells g v) =
-          map (heapgraph_cell_val (heapgraph_generations_append g gi))
-              (heapgraph_block_cells (heapgraph_generations_append g gi) v)). {
-    unfold heapgraph_block_cells. simpl. apply map_ext_in. intros.
-    destruct a; [destruct s|]; simpl; auto. rewrite heapgraph_generations_append__heapgraph_block_ptr; auto.
-    red in H1. apply (H1 v); auto. unfold heapgraph_block_fields.
-    rewrite <- filter_sum_right_In_iff. assumption. } rewrite <- H2.
-  destruct (block_mark (heapgraph_block g v)) eqn:?; auto. f_equal.
-  rewrite heapgraph_generations_append__heapgraph_block_ptr; auto. destruct (H0 _ H Heqb). assumption.
+  (intros).
+  (unfold heapgraph_block_header).
+  reflexivity.
 Qed.
 
-Lemma ang_graph_gen_size_old: forall g gi gen,
-    heapgraph_has_gen g gen -> heapgraph_generation_size g gen =
-                           heapgraph_generation_size (heapgraph_generations_append g gi) gen.
+Lemma ang_heapgraph_block_cells_vals_old :
+  forall g gi v,
+  heapgraph_has_block g v ->
+  copy_compatible g ->
+  no_dangling_dst g ->
+  heapgraph_block_cells_vals g v = heapgraph_block_cells_vals (heapgraph_generations_append g gi) v.
 Proof.
-  intros. unfold heapgraph_generation_size. rewrite heapgraph_generation__heapgraph_generations_append__old by assumption.
-  apply fold_left_ext. intros. unfold heapgraph_block_size_accum. reflexivity.
+  (intros).
+  (unfold heapgraph_block_cells_vals).
+  (simpl).
+  (assert
+    (map (heapgraph_cell_val g) (heapgraph_block_cells g v) =
+     map (heapgraph_cell_val (heapgraph_generations_append g gi))
+       (heapgraph_block_cells (heapgraph_generations_append g gi) v))).
+  {
+    (unfold heapgraph_block_cells).
+    (simpl).
+    (apply map_ext_in).
+    (intros).
+    (destruct a; [ destruct s |  ]; simpl; auto).
+    (rewrite heapgraph_generations_append__heapgraph_block_ptr; auto).
+    (red in H1).
+    (apply (H1 v); auto).
+    (unfold heapgraph_block_fields).
+    (rewrite <- filter_sum_right_In_iff).
+    assumption.
+  }
+  (rewrite <- H2).
+  (destruct (block_mark (heapgraph_block g v)) eqn:?; auto).
+  f_equal.
+  (rewrite heapgraph_generations_append__heapgraph_block_ptr; auto).
+  (destruct (H0 _ H Heqb)).
+  assumption.
 Qed.
 
-Lemma stcte_add: forall g gi i,
-    generation_block_count gi = O -> heapgraph_can_copy_except g i ->
-    heapgraph_can_copy_except (heapgraph_generations_append g gi) i.
+Lemma ang_graph_gen_size_old :
+  forall g gi gen,
+  heapgraph_has_gen g gen ->
+  heapgraph_generation_size g gen = heapgraph_generation_size (heapgraph_generations_append g gi) gen.
 Proof.
-  intros. unfold heapgraph_can_copy_except in *. intros. rewrite heapgraph_has_gen__heapgraph_generations_append in H3.
-  destruct H3.
-  - specialize (H0 _ H1 H2 H3). unfold heapgraph_generation_can_copy in *.
-    rewrite <- ang_graph_gen_size_old; assumption.
-  - unfold heapgraph_generation_can_copy. simpl. unfold heapgraph_generation_size.
-    rewrite H3 at 4. rewrite heapgraph_generation__heapgraph_generations_append__new, H. unfold heapgraph_block_size_prev.
-    simpl. destruct n. 1: contradiction. simpl. rewrite Z.sub_0_r.
-    apply generation_size_le_S.
+  (intros).
+  (unfold heapgraph_generation_size).
+  (rewrite heapgraph_generation__heapgraph_generations_append__old by assumption).
+  (apply fold_left_ext).
+  (intros).
+  (unfold heapgraph_block_size_accum).
+  reflexivity.
 Qed.
 
-Lemma graph_unmarked_add: forall g gi,
-    generation_block_count gi = O -> graph_unmarked g ->
-    graph_unmarked (heapgraph_generations_append g gi).
+Lemma stcte_add :
+  forall g gi i,
+  generation_block_count gi = O ->
+  heapgraph_can_copy_except g i -> heapgraph_can_copy_except (heapgraph_generations_append g gi) i.
 Proof.
-  intros. unfold graph_unmarked in *. intros. apply heapgraph_generations_append__heapgraph_has_block_inv in H1; auto.
-  simpl. apply H0. assumption.
+  (intros).
+  (unfold heapgraph_can_copy_except in *).
+  (intros).
+  (rewrite heapgraph_has_gen__heapgraph_generations_append in H3).
+  (destruct H3).
+  - specialize (H0 _ H1 H2 H3).
+    (unfold heapgraph_generation_can_copy in *).
+    (rewrite <- ang_graph_gen_size_old; assumption).
+  - (unfold heapgraph_generation_can_copy).
+    (simpl).
+    (unfold heapgraph_generation_size).
+    (rewrite H3  at 4).
+    (rewrite heapgraph_generation__heapgraph_generations_append__new, H).
+    (unfold heapgraph_block_size_prev).
+    (simpl).
+    (destruct n).
+    1: contradiction.
+    (simpl).
+    (rewrite Z.sub_0_r).
+    (apply generation_size_le_S).
 Qed.
 
-Lemma ang_heapgraph_block_fields: forall g gi v,
-    heapgraph_block_fields g v = heapgraph_block_fields (heapgraph_generations_append g gi) v.
-Proof. intros. unfold heapgraph_block_fields, heapgraph_block_cells. simpl. reflexivity. Qed.
-
-Lemma no_backward_edge_add: forall g gi,
-    generation_block_count gi = O -> no_backward_edge g ->
-    no_backward_edge (heapgraph_generations_append g gi).
+Lemma graph_unmarked_add :
+  forall g gi, generation_block_count gi = O -> graph_unmarked g -> graph_unmarked (heapgraph_generations_append g gi).
 Proof.
-  intros. unfold no_backward_edge, gen2gen_no_edge in *. intros. simpl.
-  pose proof (heapgraph_has_field__in H2) as Hfield.
-  rewrite <- ang_heapgraph_block_fields in Hfield.
-  pose proof (heapgraph_has_field__has_block H2) as Hblock.
-  apply heapgraph_generations_append__heapgraph_has_block_inv in Hblock; auto.
-  apply H0; auto.
-  split; simpl; auto.
+  (intros).
+  (unfold graph_unmarked in *).
+  (intros).
+  (apply heapgraph_generations_append__heapgraph_has_block_inv in H1; auto).
+  (simpl).
+  (apply H0).
+  assumption.
 Qed.
 
-Lemma no_dangling_dst_add: forall g gi,
-    generation_block_count gi = O -> no_dangling_dst g ->
-    no_dangling_dst (heapgraph_generations_append g gi).
+Lemma ang_heapgraph_block_fields :
+  forall g gi v, heapgraph_block_fields g v = heapgraph_block_fields (heapgraph_generations_append g gi) v.
 Proof.
-  intros. unfold no_dangling_dst in *. intros. simpl.
-  apply heapgraph_generations_append__heapgraph_has_block_inv in H1; auto. rewrite <- ang_heapgraph_block_fields in H2.
-  apply heapgraph_generations_append__heapgraph_has_block, (H0 v); auto.
+  (intros).
+  (unfold heapgraph_block_fields, heapgraph_block_cells).
+  (simpl).
+  reflexivity.
 Qed.
 
-
-Lemma lgd_heapgraph_has_block (g: HeapGraph) (e: Field) (v v': Addr):
-    heapgraph_has_block g v <-> heapgraph_has_block (labeledgraph_gen_dst g e v') v.
+Lemma no_backward_edge_add :
+  forall g gi,
+  generation_block_count gi = O -> no_backward_edge g -> no_backward_edge (heapgraph_generations_append g gi).
 Proof.
-    split ; intro H ; destruct H ; now constructor.
+  (intros).
+  (unfold no_backward_edge, gen2gen_no_edge in *).
+  (intros).
+  (simpl).
+  (pose proof (heapgraph_has_field__in H2) as Hfield).
+  (rewrite <- ang_heapgraph_block_fields in Hfield).
+  (pose proof (heapgraph_has_field__has_block H2) as Hblock).
+  (apply heapgraph_generations_append__heapgraph_has_block_inv in Hblock; auto).
+  (apply H0; auto).
+  (split; simpl; auto).
 Qed.
 
-Lemma lgd_graph_has_gen: forall g e v x,
-    heapgraph_has_gen (labeledgraph_gen_dst g e v) x <-> heapgraph_has_gen g x.
-Proof. intros; unfold heapgraph_has_gen; intuition. Qed.
-
-Lemma lgd_raw_fld_length_eq: forall (g: HeapGraph) v e v',
-    Zlength (block_fields (heapgraph_block g v)) =
-    Zlength (block_fields (heapgraph_block (labeledgraph_gen_dst g e v') v)).
-Proof. reflexivity. Qed.
-
-Lemma lgd_heapgraph_block_ptr_eq: forall g e v' x,
-    heapgraph_block_ptr (labeledgraph_gen_dst g e v') x = heapgraph_block_ptr g x.
-Proof. reflexivity. Qed.
-
-Lemma lgd_heapgraph_block_cells_eq: forall (g : HeapGraph) (v v': Addr) e,
-    heapgraph_block_cells (labeledgraph_gen_dst g e v') v = heapgraph_block_cells g v.
-Proof. reflexivity. Qed.
-
-Lemma heapgraph_block_header__labeledgraph_gen_dst: forall g e v' x,
-    heapgraph_block_header g x = heapgraph_block_header (labeledgraph_gen_dst g e v') x.
-Proof. reflexivity. Qed.
-
-Lemma lgd_block_mark_eq: forall (g: HeapGraph) e (v v' : Addr),
-    block_mark (heapgraph_block g v) = block_mark (heapgraph_block (labeledgraph_gen_dst g e v') v).
-Proof. reflexivity. Qed.
-
-Lemma lgd_dst_old: forall (g: HeapGraph) e v e',
-    e <> e' -> dst (labeledgraph_gen_dst g e v) e' = dst g e'.
+Lemma no_dangling_dst_add :
+  forall g gi,
+  generation_block_count gi = O -> no_dangling_dst g -> no_dangling_dst (heapgraph_generations_append g gi).
 Proof.
-  intros. simpl. unfold updateEdgeFunc. rewrite if_false. 1: reflexivity. auto.
+  (intros).
+  (unfold no_dangling_dst in *).
+  (intros).
+  (simpl).
+  (apply heapgraph_generations_append__heapgraph_has_block_inv in H1; auto).
+  (rewrite <- ang_heapgraph_block_fields in H2).
+  (apply heapgraph_generations_append__heapgraph_has_block, (H0 v); auto).
 Qed.
 
-Lemma lgd_dst_new: forall (g: HeapGraph) e v,
-    dst (labeledgraph_gen_dst g e v) e = v.
-Proof. intros. simpl. unfold updateEdgeFunc. rewrite if_true; reflexivity. Qed.
+Lemma lgd_heapgraph_has_block 
+  (g : HeapGraph) (e : Field) 
+  (v v' : Addr) : heapgraph_has_block g v <-> heapgraph_has_block (labeledgraph_gen_dst g e v') v.
+Proof.
+  (split; intro H; destruct H; now constructor).
+Qed.
 
-Definition closure_has_index (g: HeapGraph) (gen index: nat) :=
+Lemma lgd_graph_has_gen : forall g e v x, heapgraph_has_gen (labeledgraph_gen_dst g e v) x <-> heapgraph_has_gen g x.
+Proof.
+  (intros; unfold heapgraph_has_gen; intuition).
+Qed.
+
+Lemma lgd_raw_fld_length_eq :
+  forall (g : HeapGraph) v e v',
+  Zlength (block_fields (heapgraph_block g v)) =
+  Zlength (block_fields (heapgraph_block (labeledgraph_gen_dst g e v') v)).
+Proof.
+  reflexivity.
+Qed.
+
+Lemma lgd_heapgraph_block_ptr_eq :
+  forall g e v' x, heapgraph_block_ptr (labeledgraph_gen_dst g e v') x = heapgraph_block_ptr g x.
+Proof.
+  reflexivity.
+Qed.
+
+Lemma lgd_heapgraph_block_cells_eq :
+  forall (g : HeapGraph) (v v' : Addr) e,
+  heapgraph_block_cells (labeledgraph_gen_dst g e v') v = heapgraph_block_cells g v.
+Proof.
+  reflexivity.
+Qed.
+
+Lemma heapgraph_block_header__labeledgraph_gen_dst :
+  forall g e v' x, heapgraph_block_header g x = heapgraph_block_header (labeledgraph_gen_dst g e v') x.
+Proof.
+  reflexivity.
+Qed.
+
+Lemma lgd_block_mark_eq :
+  forall (g : HeapGraph) e (v v' : Addr),
+  block_mark (heapgraph_block g v) = block_mark (heapgraph_block (labeledgraph_gen_dst g e v') v).
+Proof.
+  reflexivity.
+Qed.
+
+Lemma lgd_dst_old : forall (g : HeapGraph) e v e', e <> e' -> dst (labeledgraph_gen_dst g e v) e' = dst g e'.
+Proof.
+  (intros).
+  (simpl).
+  (unfold updateEdgeFunc).
+  (rewrite if_false).
+  1: reflexivity.
+  auto.
+Qed.
+
+Lemma lgd_dst_new : forall (g : HeapGraph) e v, dst (labeledgraph_gen_dst g e v) e = v.
+Proof.
+  (intros).
+  (simpl).
+  (unfold updateEdgeFunc).
+  (rewrite if_true; reflexivity).
+Qed.
+
+Definition closure_has_index 
+  (g : HeapGraph) (gen index : nat) := 
   (index <= generation_block_count (heapgraph_generation g gen))%nat.
 
-Definition closure_has_v (g: HeapGraph) (v: Addr): Prop :=
+Definition closure_has_v 
+  (g : HeapGraph) (v : Addr) : Prop :=
   heapgraph_has_gen g (addr_gen v) /\ closure_has_index g (addr_gen v) (addr_block v).
 
-Lemma heapgraph_has_block_in_closure (g : HeapGraph) (v : Addr)
-    (Hv: heapgraph_has_block g v):
-    closure_has_v g v.
+Lemma heapgraph_has_block_in_closure (g : HeapGraph) (v : Addr) (Hv : heapgraph_has_block g v) : closure_has_v g v.
 Proof.
-    destruct v as [gen index].
-    destruct Hv.
-    unfold closure_has_v, closure_has_index.
-    intuition.
+  (destruct v as [gen index]).
+  (destruct Hv).
+  (unfold closure_has_v, closure_has_index).
+  intuition.
 Qed.
 
-
-Lemma lgd_f2v_eq_except_one: forall g fd e v',
-    fd <> (inr e) ->
-    heapgraph_cell_val g fd = heapgraph_cell_val (labeledgraph_gen_dst g e v') fd.
+Lemma lgd_f2v_eq_except_one :
+  forall g fd e v', fd <> inr e -> heapgraph_cell_val g fd = heapgraph_cell_val (labeledgraph_gen_dst g e v') fd.
 Proof.
-  intros; unfold heapgraph_cell_val; simpl.
-  destruct fd; [destruct s|]; try reflexivity.
-  unfold updateEdgeFunc; if_tac; [exfalso; apply H; rewrite H0|]; reflexivity.
+  (intros; unfold heapgraph_cell_val; simpl).
+  (destruct fd; [ destruct s |  ]; try reflexivity).
+  (unfold updateEdgeFunc; if_tac; [ exfalso; apply H; rewrite H0 |  ]; reflexivity).
 Qed.
 
-Lemma lgd_map_f2v_diff_vert_eq: forall g v v' v1 e n,
-    0 <= n < Zlength (heapgraph_block_cells g v) ->
-    Znth n (heapgraph_block_cells g v) = inr e ->
-    v1 <> v ->
-    map (heapgraph_cell_val g) (heapgraph_block_cells g v1) =
-    map (heapgraph_cell_val (labeledgraph_gen_dst g e v'))
-        (heapgraph_block_cells (labeledgraph_gen_dst g e v') v1).
+Lemma lgd_map_f2v_diff_vert_eq :
+  forall g v v' v1 e n,
+  0 <= n < Zlength (heapgraph_block_cells g v) ->
+  Znth n (heapgraph_block_cells g v) = inr e ->
+  v1 <> v ->
+  map (heapgraph_cell_val g) (heapgraph_block_cells g v1) =
+  map (heapgraph_cell_val (labeledgraph_gen_dst g e v')) (heapgraph_block_cells (labeledgraph_gen_dst g e v') v1).
 Proof.
-    intros.
-    rewrite lgd_heapgraph_block_cells_eq.
-    apply Znth_list_eq. split.
-    1: repeat rewrite Zlength_map; reflexivity.
-    intros. rewrite Zlength_map in H2.
-    repeat rewrite Znth_map by assumption.
-    apply lgd_f2v_eq_except_one. intro.
-    pose proof (heapgraph_block_cells_edge_unique g e v
-                                        v1 n j H H2 H0 H3).
-    destruct H4. unfold not in H1. symmetry in H5.
-    apply (H1 H5).
+  (intros).
+  (rewrite lgd_heapgraph_block_cells_eq).
+  (apply Znth_list_eq).
+  split.
+  1: (repeat rewrite Zlength_map; reflexivity).
+  (intros).
+  (rewrite Zlength_map in H2).
+  (repeat rewrite Znth_map by assumption).
+  (apply lgd_f2v_eq_except_one).
+  intro.
+  (pose proof (heapgraph_block_cells_edge_unique g e v v1 n j H H2 H0 H3)).
+  (destruct H4).
+  (unfold not in H1).
+  symmetry in H5.
+  (apply (H1 H5)).
 Qed.
 
-Lemma lgd_f2v_eq_after_update: forall g v v' e n j,
+Lemma lgd_f2v_eq_after_update :
+  forall g v v' e n j,
   0 <= n < Zlength (heapgraph_block_cells g v) ->
   0 <= j < Zlength (heapgraph_block_cells g v) ->
   Znth n (heapgraph_block_cells g v) = inr e ->
-  Znth j (upd_Znth n (map (heapgraph_cell_val g)
-                          (heapgraph_block_cells g v)) (heapgraph_block_ptr g v')) =
+  Znth j (upd_Znth n (map (heapgraph_cell_val g) (heapgraph_block_cells g v)) (heapgraph_block_ptr g v')) =
   Znth j
-    (map (heapgraph_cell_val (labeledgraph_gen_dst g e v'))
-         (heapgraph_block_cells (labeledgraph_gen_dst g e v') v)).
+    (map (heapgraph_cell_val (labeledgraph_gen_dst g e v')) (heapgraph_block_cells (labeledgraph_gen_dst g e v') v)).
 Proof.
-  intros.
-  rewrite Znth_map.
-  2: rewrite lgd_heapgraph_block_cells_eq; assumption.
-  assert (j = n \/ j <> n) by lia; destruct H2.
-  + subst j; rewrite upd_Znth_same.
-    2: rewrite Zlength_map; assumption.
-    replace (heapgraph_block_cells (labeledgraph_gen_dst g e v') v)
-      with (heapgraph_block_cells g v) by reflexivity.
-    rewrite H1; simpl heapgraph_cell_val.
-    unfold updateEdgeFunc; if_tac; try reflexivity.
-    unfold complement in H2; assert (e = e) by reflexivity.
-    apply H2 in H3; exfalso; assumption.
-  + rewrite upd_Znth_diff_strong; [|rewrite Zlength_map|]; try assumption.
-    rewrite Znth_map by assumption.
-    apply (lgd_f2v_eq_except_one g (Znth j (heapgraph_block_cells g v))).
-    intro. pose proof (heapgraph_block_cells_edge_unique g e v v n j H H0 H1 H3).
+  (intros).
+  (rewrite Znth_map).
+  2: (rewrite lgd_heapgraph_block_cells_eq; assumption).
+  (assert (j = n \/ j <> n) by lia; destruct H2).
+  + (subst j; rewrite upd_Znth_same).
+    2: (rewrite Zlength_map; assumption).
+    replace (heapgraph_block_cells (labeledgraph_gen_dst g e v') v) with (heapgraph_block_cells g v) by reflexivity.
+    (rewrite H1; simpl heapgraph_cell_val).
+    (unfold updateEdgeFunc; if_tac; try reflexivity).
+    (unfold complement in H2; assert (e = e) by reflexivity).
+    (apply H2 in H3; exfalso; assumption).
+  + (rewrite upd_Znth_diff_strong; [  | rewrite Zlength_map |  ]; try assumption).
+    (rewrite Znth_map by assumption).
+    (apply (lgd_f2v_eq_except_one g (Znth j (heapgraph_block_cells g v)))).
+    intro.
+    (pose proof (heapgraph_block_cells_edge_unique g e v v n j H H0 H1 H3)).
     lia.
 Qed.
 
-Lemma lgd_mfv_change_in_one_spot: forall g v e v' n,
-    0 <= n < Zlength (heapgraph_block_cells g v) ->
-    block_mark (heapgraph_block g v) = false ->
-    Znth n (heapgraph_block_cells g v) = inr e ->
-    upd_Znth n (heapgraph_block_cells_vals g v) (heapgraph_block_ptr g v') =
-    (heapgraph_block_cells_vals (labeledgraph_gen_dst g e v') v).
+Lemma lgd_mfv_change_in_one_spot :
+  forall g v e v' n,
+  0 <= n < Zlength (heapgraph_block_cells g v) ->
+  block_mark (heapgraph_block g v) = false ->
+  Znth n (heapgraph_block_cells g v) = inr e ->
+  upd_Znth n (heapgraph_block_cells_vals g v) (heapgraph_block_ptr g v') =
+  heapgraph_block_cells_vals (labeledgraph_gen_dst g e v') v.
 Proof.
-  intros.
-  rewrite (Znth_list_eq (upd_Znth n (heapgraph_block_cells_vals g v)
-               (heapgraph_block_ptr g v')) (heapgraph_block_cells_vals
-                     (labeledgraph_gen_dst g e v') v)).
-  rewrite upd_Znth_Zlength, fields_eq_length.
-  2: rewrite fields_eq_length; rewrite heapgraph_block_cells_eq_length in H; assumption.
-  split. 1: rewrite fields_eq_length; reflexivity.
-  intros.
-  unfold heapgraph_block_cells_vals.
-  replace (block_mark (heapgraph_block (labeledgraph_gen_dst g e v') v))
-    with (block_mark (heapgraph_block g v)) by reflexivity.
-  rewrite H0; rewrite <- heapgraph_block_cells_eq_length in H2.
-  apply lgd_f2v_eq_after_update; assumption.
+  (intros).
+  (rewrite
+    (Znth_list_eq (upd_Znth n (heapgraph_block_cells_vals g v) (heapgraph_block_ptr g v'))
+       (heapgraph_block_cells_vals (labeledgraph_gen_dst g e v') v))).
+  (rewrite upd_Znth_Zlength, fields_eq_length).
+  2: (rewrite fields_eq_length; rewrite heapgraph_block_cells_eq_length in H; assumption).
+  split.
+  1: (rewrite fields_eq_length; reflexivity).
+  (intros).
+  (unfold heapgraph_block_cells_vals).
+  replace (block_mark (heapgraph_block (labeledgraph_gen_dst g e v') v)) with 
+   (block_mark (heapgraph_block g v)) 
+   by reflexivity.
+  (rewrite H0; rewrite <- heapgraph_block_cells_eq_length in H2).
+  (apply lgd_f2v_eq_after_update; assumption).
 Qed.
 
-Lemma lgd_no_dangling_dst: forall g e v',
-    heapgraph_has_block g v' ->
-    no_dangling_dst g ->
-     no_dangling_dst (labeledgraph_gen_dst g e v').
+Lemma lgd_no_dangling_dst :
+  forall g e v', heapgraph_has_block g v' -> no_dangling_dst g -> no_dangling_dst (labeledgraph_gen_dst g e v').
 Proof.
-  intros. unfold no_dangling_dst in *.
-  intros. rewrite <- lgd_heapgraph_has_block.
-  simpl.
-  unfold updateEdgeFunc ; if_tac ; [assumption | apply (H0 v)] ; try assumption.
-  destruct H1 ; simpl in * ; now constructor.
+  (intros).
+  (unfold no_dangling_dst in *).
+  (intros).
+  (rewrite <- lgd_heapgraph_has_block).
+  (simpl).
+  (unfold updateEdgeFunc; if_tac; [ assumption | apply (H0 v) ]; try assumption).
+  (destruct H1; simpl in *; now constructor).
 Qed.
 
-Lemma lgd_no_dangling_dst_copied_vert: forall g e v,
-    copy_compatible g ->
-    heapgraph_has_block g v ->
-    block_mark (heapgraph_block g v) = true ->
-    no_dangling_dst g ->
-    no_dangling_dst (labeledgraph_gen_dst g e (block_copied_vertex (heapgraph_block g v))).
+Lemma lgd_no_dangling_dst_copied_vert :
+  forall g e v,
+  copy_compatible g ->
+  heapgraph_has_block g v ->
+  block_mark (heapgraph_block g v) = true ->
+  no_dangling_dst g -> no_dangling_dst (labeledgraph_gen_dst g e (block_copied_vertex (heapgraph_block g v))).
 Proof.
-  intros.
-  assert (heapgraph_has_block g (block_copied_vertex (heapgraph_block g v))) by apply (H v H0 H1).
-  apply lgd_no_dangling_dst; assumption.
+  (intros).
+  (assert (heapgraph_has_block g (block_copied_vertex (heapgraph_block g v))) by apply (H v H0 H1)).
+  (apply lgd_no_dangling_dst; assumption).
 Qed.
 
-
-Lemma block_mark__false_prep64: forall z,
-    0 <= z < two_p (8 * 8) ->
-    Int64.and (Int64.repr z) (Int64.repr 255) =
-    Int64.sub (Int64.repr z)
-              (Int64.mul (Int64.repr (z / two_p 8)) (Int64.repr (two_p 8))).
+Lemma block_mark__false_prep64 :
+  forall z,
+  0 <= z < two_p (8 * 8) ->
+  Int64.and (Int64.repr z) (Int64.repr 255) =
+  Int64.sub (Int64.repr z) (Int64.mul (Int64.repr (z / two_p 8)) (Int64.repr (two_p 8))).
 Proof.
-  intros. replace (Int64.repr 255) with (Int64.sub (Int64.repr 256) Int64.one) by
-      now vm_compute.
-  rewrite <- (Int64.modu_and _ _ (Int64.repr 8)) by now vm_compute.
-  rewrite Int64.modu_divu by (vm_compute; intro S; inversion S).
-  rewrite (Int64.divu_pow2 _ _ (Int64.repr 8)) by now vm_compute.
-  rewrite (Int64.mul_pow2 _ _ (Int64.repr 8)) by now vm_compute.
-  rewrite Int64.shru_div_two_p, !Int64.unsigned_repr; [| rep_lia | ].
-  - rewrite Int64.shl_mul_two_p, Int64.unsigned_repr by rep_lia. easy.
-  - simpl Z.mul in H. unfold Int64.max_unsigned, Int64.modulus.
-    unfold Int64.wordsize, Wordsize_64.wordsize. rewrite two_power_nat_two_p.
-    simpl Z.of_nat. lia.
+  (intros).
+  replace (Int64.repr 255) with (Int64.sub (Int64.repr 256) Int64.one) by now vm_compute.
+  (rewrite <- (Int64.modu_and _ _ (Int64.repr 8)) by now vm_compute).
+  (rewrite Int64.modu_divu by (vm_compute; intro S; inversion S)).
+  (rewrite (Int64.divu_pow2 _ _ (Int64.repr 8)) by now vm_compute).
+  (rewrite (Int64.mul_pow2 _ _ (Int64.repr 8)) by now vm_compute).
+  (rewrite Int64.shru_div_two_p, !Int64.unsigned_repr; [  | rep_lia |  ]).
+  - (rewrite Int64.shl_mul_two_p, Int64.unsigned_repr by rep_lia).
+    easy.
+  - (simpl Z.mul in H).
+    (unfold Int64.max_unsigned, Int64.modulus).
+    (unfold Int64.wordsize, Wordsize_64.wordsize).
+    (rewrite two_power_nat_two_p).
+    (simpl Z.of_nat).
+    lia.
 Qed.
 
-Lemma block_mark__false_prep32: forall z,
-    0 <= z < two_p (4 * 8) ->
-    Int.and (Int.repr z) (Int.repr 255) =
-    Int.sub (Int.repr z)
-              (Int.mul (Int.repr (z / two_p 8)) (Int.repr (two_p 8))).
+Lemma block_mark__false_prep32 :
+  forall z,
+  0 <= z < two_p (4 * 8) ->
+  Int.and (Int.repr z) (Int.repr 255) = Int.sub (Int.repr z) (Int.mul (Int.repr (z / two_p 8)) (Int.repr (two_p 8))).
 Proof.
-  intros. replace (Int.repr 255) with (Int.sub (Int.repr 256) Int.one) by
-      now vm_compute.
-  rewrite <- (Int.modu_and _ _ (Int.repr 8)) by now vm_compute.
-  rewrite Int.modu_divu by (vm_compute; intro S; inversion S).
-  rewrite (Int.divu_pow2 _ _ (Int.repr 8)) by now vm_compute.
-  rewrite (Int.mul_pow2 _ _ (Int.repr 8)) by now vm_compute.
-  rewrite Int.shru_div_two_p, !Int.unsigned_repr; [| rep_lia | ].
-  - rewrite Int.shl_mul_two_p, Int.unsigned_repr by rep_lia. easy.
-  - simpl Z.mul in H. unfold Int.max_unsigned, Int.modulus.
-    unfold Int.wordsize, Wordsize_32.wordsize. rewrite two_power_nat_two_p.
-    simpl Z.of_nat. lia.
+  (intros).
+  replace (Int.repr 255) with (Int.sub (Int.repr 256) Int.one) by now vm_compute.
+  (rewrite <- (Int.modu_and _ _ (Int.repr 8)) by now vm_compute).
+  (rewrite Int.modu_divu by (vm_compute; intro S; inversion S)).
+  (rewrite (Int.divu_pow2 _ _ (Int.repr 8)) by now vm_compute).
+  (rewrite (Int.mul_pow2 _ _ (Int.repr 8)) by now vm_compute).
+  (rewrite Int.shru_div_two_p, !Int.unsigned_repr; [  | rep_lia |  ]).
+  - (rewrite Int.shl_mul_two_p, Int.unsigned_repr by rep_lia).
+    easy.
+  - (simpl Z.mul in H).
+    (unfold Int.max_unsigned, Int.modulus).
+    (unfold Int.wordsize, Wordsize_32.wordsize).
+    (rewrite two_power_nat_two_p).
+    (simpl Z.of_nat).
+    lia.
 Qed.
 
-Lemma block_mark__false: forall g v,
-    block_mark (heapgraph_block g v) = false ->
-    if Archi.ptr64 then
-        Int64.and (Int64.repr (heapgraph_block_header g v)) (Int64.repr 255) =
-        Int64.repr (block_tag (heapgraph_block g v))
-    else Int.and (Int.repr (heapgraph_block_header g v)) (Int.repr 255) =
-         Int.repr (block_tag (heapgraph_block g v)).
+Lemma block_mark__false :
+  forall g v,
+  block_mark (heapgraph_block g v) = false ->
+  if Archi.ptr64
+  then
+   Int64.and (Int64.repr (heapgraph_block_header g v)) (Int64.repr 255) = Int64.repr (block_tag (heapgraph_block g v))
+  else Int.and (Int.repr (heapgraph_block_header g v)) (Int.repr 255) = Int.repr (block_tag (heapgraph_block g v)).
 Proof.
-  intros. cbv delta [Archi.ptr64]. simpl.
-  first [rewrite block_mark__false_prep32 | rewrite block_mark__false_prep64].
-  2: apply heapgraph_block_header__range.
-  unfold heapgraph_block_header in *. remember (heapgraph_block g v) as r eqn:E. clear E.
-  rewrite H, !Zbits.Zshiftl_mul_two_p in * by lia. rewrite <- Z.add_assoc.
-  replace (block_color r * two_p 8 + Zlength (block_fields r) * two_p 10)
-    with ((block_color r + Zlength (block_fields r) * two_p 2) * two_p 8) by
-      (rewrite Z.mul_add_distr_r, <- Z.mul_assoc, <- two_p_is_exp by lia;
-       reflexivity). rewrite Z.div_add by (vm_compute; intros S; inversion S).
-  assert (block_tag r / two_p 8 = 0) by (apply Z.div_small, block_tag__range).
-  rewrite H0, Z.add_0_l.
-  first [rewrite mul_repr, sub_repr | rewrite mul64_repr, sub64_repr].
+  (intros).
+  (cbv delta [Archi.ptr64]).
+  (simpl).
+  (first [ rewrite block_mark__false_prep32 | rewrite block_mark__false_prep64 ]).
+  2: (apply heapgraph_block_header__range).
+  (unfold heapgraph_block_header in *).
+  (remember (heapgraph_block g v) as r eqn:E ).
+  clear E.
+  (rewrite H, !Zbits.Zshiftl_mul_two_p in * by lia).
+  (rewrite <- Z.add_assoc).
+  replace (block_color r * two_p 8 + Zlength (block_fields r) * two_p 10) with
+   ((block_color r + Zlength (block_fields r) * two_p 2) * two_p 8)
+   by (rewrite Z.mul_add_distr_r, <- Z.mul_assoc, <- two_p_is_exp by lia; reflexivity).
+  (rewrite Z.div_add by (vm_compute; intros S; inversion S)).
+  (assert (block_tag r / two_p 8 = 0) by apply Z.div_small, block_tag__range).
+  (rewrite H0, Z.add_0_l).
+  (first [ rewrite mul_repr, sub_repr | rewrite mul64_repr, sub64_repr ]).
   now rewrite <- Z.add_sub_assoc, Z.sub_diag, Z.add_0_r.
 Qed.
 
+Definition root_t : Type := Z + GC_Pointer + Addr.
 
-Definition root_t: Type := Z + GC_Pointer + Addr.
+Instance root_t_inhabitant : (Inhabitant root_t) := (inl (inl Z.zero)).
 
-Instance root_t_inhabitant: Inhabitant root_t := inl (inl Z.zero).
-
-
-Definition root2val (g: HeapGraph) (fd: root_t) : val :=
+Definition root2val (g : HeapGraph) 
+  (fd : root_t) : val :=
   match fd with
   | inl (inl z) => odd_Z2val z
   | inl (inr p) => GC_Pointer2val p
   | inr v => heapgraph_block_ptr g v
   end.
 
+Definition roots_t : Type := list root_t.
 
-Definition roots_t: Type := list root_t.
-
-Lemma root_in_outlier: forall (roots: roots_t) outlier p,
-    In (inl (inr p)) roots ->
-    incl (filter_sum_right (filter_sum_left roots)) outlier -> In p outlier.
+Lemma root_in_outlier :
+  forall (roots : roots_t) outlier p,
+  In (inl (inr p)) roots -> incl (filter_sum_right (filter_sum_left roots)) outlier -> In p outlier.
 Proof.
-  intros. apply H0. rewrite <- filter_sum_right_In_iff, <- filter_sum_left_In_iff.
+  (intros).
+  (apply H0).
+  (rewrite <- filter_sum_right_In_iff, <- filter_sum_left_In_iff).
   assumption.
 Qed.
 
-Definition roots_have_no_gen (roots: roots_t) (gen: nat): Prop :=
-  forall v, In (inr v) roots -> addr_gen v <> gen.
+Definition roots_have_no_gen (roots : roots_t) (gen : nat) : Prop := forall v, In (inr v) roots -> addr_gen v <> gen.
 
-Definition outlier_t: Type := list GC_Pointer.
-
+Definition outlier_t : Type := list GC_Pointer.
